Split FMapTrie proofs and definitions for positivity checker (#1273)
* Split FMapTrie proofs and definitions for positivity checker

* Split up the shape module

* Fix trie shape ind so that it's actually true

src/Util/FSets/FMapTrie.v
@@ -5,7 +5,6 @@
 (** This module implements tries.
     It follows the implementation from Coq's clib, to some extent.
 *)
-Require Import Coq.Program.Program.
 Require Import Coq.Bool.Bool.
 Require Import Coq.Lists.List.
 Require Import Coq.Structures.Orders.
@@ -38,6 +37,9 @@ Require Import Crypto.Util.Tactics.InHypUnderBindersDo.
 Require Import Crypto.Util.Tactics.Head.
 Require Import Crypto.Util.Tactics.BreakMatch.
 Require Import Crypto.Util.Tactics.SetoidSubst.
+Require Import Crypto.Util.FSets.FMapTrie.Shape.
+Import TrieTactics.
+Import EverythingGen.
 
 Local Set Implicit Arguments.
 Local Set Primitive Projections.
@@ -50,371 +52,6 @@ Local Open Scope bool_scope.
 Local Open Scope lazy_bool_scope.
 Local Open Scope type_scope.
 Local Open Scope list_scope.
-
-Module Type TypFunctor.
-  Parameter t : Type -> Type.
-End TypFunctor.
-
-Module Import EverythingGen.
-  Polymorphic Definition id_fix {T} (x : T) := x.
-  Polymorphic Definition id_fix_2 {T} (x : T) := x.
-  Polymorphic Definition id_case {T} (x : T) := x.
-  Section __.
-    Context (t : Type -> Type)
-            (map_key : Type)
-            (map_t : Type -> Type)
-            (map_empty : forall elt, map_t elt)
-            (map_is_empty : forall elt, map_t elt -> bool)
-            (map_NonEmpty : forall elt, map_t elt -> Prop)
-            (map_is_empty_1 : forall elt m, @map_is_empty elt m = false -> @map_NonEmpty elt m)
-            (map_fold : forall elt A : Type, (map_key -> elt -> A -> A) -> map_t elt -> A -> A)
-            (map_mapi : forall elt elt' : Type, (map_key -> elt -> elt') -> map_t elt -> map_t elt')
-            (map_mapi_nonEmpty : forall elt elt' f m, @map_NonEmpty _ m -> @map_NonEmpty _ (@map_mapi elt elt' f m))
-            (map_map2 : forall elt elt' elt'' : Type, (option elt -> option elt' -> option elt'') -> map_t elt -> map_t elt' -> map_t elt'')
-            (map_find : forall elt : Type, map_key -> map_t elt -> option elt).
-
-    Local Notation t' elt := (option (t elt)).
-    Local Notation node_NonEmpty x y := match x, y with None, None => False | _, _ => True end.
-    Local Notation node_NonEmpty' x y := match y, x with None, None => False | _, _ => True end.
-    Local Notation map_t_t elt := { m : map_t (t elt) | map_NonEmpty m }.
-
-    Section step.
-      Context (Node : forall elt (d : option elt) (m : option (map_t_t elt)), node_NonEmpty d m -> t elt)
-              (t_case_nd : forall (elt : Type) (P : Type),
-                  (forall (v : option elt) (m : option (map_t_t elt)), node_NonEmpty v m -> P)
-                  -> t elt -> P)
-              (map_xmap2_l : forall elt elt' elt'', (option elt -> option elt' -> option elt'') -> map_t elt -> map_t elt'')
-              (map_xmap2_r : forall elt elt' elt'', (option elt -> option elt' -> option elt'') -> map_t elt' -> map_t elt'').
-
-      Local Arguments Node {_} _ _ _.
-
-      Definition empty' : forall elt, t' elt
-        := fun _ => None.
-
-      Definition mapi_step elt elt'
-                 (mapi : (list map_key -> elt -> elt') -> t elt -> t elt')
-                 (f : list map_key -> elt -> elt')
-        : t elt -> t elt'
-        := let d_of d := option_map (f nil) d in
-           let m_of m
-             := option_map
-                  (fun '(exist d m)
-                   => exist
-                        _
-                        (@map_mapi _ _ (fun k => mapi (fun ks => f (k :: ks))) d)
-                        (map_mapi_nonEmpty _ m))
-                  m in
-           t_case_nd
-             (fun d m pf
-              => Node
-                   (d_of d) (m_of m)
-                   (match d, m return node_NonEmpty d m -> node_NonEmpty (d_of d) (m_of m) with
-                    | None, None => fun pf => pf
-                    | _, _ => fun 'I => I
-                    end pf)).
-
-      Definition dec_empty_cps elt (m : map_t elt) T (k : option { m : map_t elt | map_NonEmpty m } -> T) : T
-        := match map_is_empty m as b return (b = false -> map_NonEmpty m) -> T with
-           | true => fun _ => k None
-           | false => fun pf => k (Some (exist _ m (pf eq_refl)))
-           end (@map_is_empty_1 _ m).
-      Local Notation dec_empty m := (@dec_empty_cps _ m _ (fun x => x)).
-      Lemma dec_empty_Some elt (m : map_t elt) v
-        : dec_empty m = Some v -> m = proj1_sig v.
-      Proof using Type.
-        cbv [dec_empty_cps].
-        generalize (@map_is_empty_1 _ m).
-        break_innermost_match; cbn; intros; inversion_option; subst; cbn; reflexivity.
-      Qed.
-      Lemma dec_empty_None elt (m : map_t elt)
-        : dec_empty m = None -> map_is_empty m = true.
-      Proof using Type.
-        cbv [dec_empty_cps].
-        generalize (@map_is_empty_1 _ m).
-        break_innermost_match; intros; inversion_option; reflexivity.
-      Qed.
-
-      Definition map2_step
-                 elt elt' elt'' (f : option elt -> option elt' -> option elt'')
-                 (map2_l : t elt -> t' elt'')
-                 (map2_r : t elt' -> t' elt'')
-                 (map2 : t elt -> t elt' -> t' elt'')
-                 (m1 : t elt) (m2 : t elt')
-        : t' elt''
-        := let F := (fun m1 m2
-                     => match m1, m2 with
-                        | Some m1, Some m2 => map2 m1 m2
-                        | Some m1, None => map2_l m1
-                        | None, Some m2 => map2_r m2
-                        | None, None => None
-                        end) in
-           let f' x y := match x, y with
-                         | None, None => None
-                         | x, y => f x y
-                         end in
-           t_case_nd
-             (fun d1 m1 pf1
-              => t_case_nd
-                   (fun d2 m2 pf2
-                    => let m := match m1, m2 with
-                                | Some (exist m1 pm1), Some (exist m2 pm2)
-                                  => dec_empty (@map_map2 _ _ _ F m1 m2)
-                                | Some (exist m1 pm1), None
-                                  => dec_empty (map_xmap2_l F m1)
-                                | None, Some (exist m2 pm2)
-                                  => dec_empty (map_xmap2_r F m2)
-                                | None, None => None
-                                end in
-                       match f' d1 d2, m with
-                       | None, None => None
-                       | d, m => Some (Node d m I)
-                       end)
-                   m2)
-             m1.
-      Definition map2_l_step
-                 elt elt' elt'' (f : option elt -> option elt' -> option elt'')
-                 (map2_l : t elt -> t' elt'')
-                 (m1 : t elt)
-        : t' elt''
-        := let f' x y := match x, y with
-                         | None, None => None
-                         | x, y => f x y
-                         end in
-           t_case_nd
-             (fun d1 m1 pf1
-              => let m := match m1 with
-                          | Some (exist m1 pm1)
-                            => dec_empty
-                                 (@map_xmap2_l
-                                    (t elt) (t elt') (t elt'')
-                                    (fun m1 _ => match m1 with
-                                                 | None => None
-                                                 | Some m1 => map2_l m1
-                                                 end)
-                                    m1)
-                          | None => None
-                          end in
-                 match f' d1 None, m with
-                 | None, None => None
-                 | d, m => Some (Node d m I)
-                 end)
-             m1.
-      Definition map2_r_step
-                 elt elt' elt'' (f : option elt -> option elt' -> option elt'')
-                 (map2_r : t elt' -> t' elt'')
-                 (m2 : t elt')
-        : t' elt''
-        := let f' x y := match x, y with
-                         | None, None => None
-                         | x, y => f x y
-                         end in
-           t_case_nd
-             (fun d2 m2 pf2
-              => let m := match m2 with
-                          | Some (exist m2 pm2)
-                            => dec_empty
-                                 (@map_xmap2_r
-                                    (t elt) (t elt') (t elt'')
-                                    (fun _ m2 => match m2 with
-                                                 | None => None
-                                                 | Some m2 => map2_r m2
-                                                 end)
-                                    m2)
-                          | None => None
-                          end in
-                 match f' None d2, m with
-                 | None, None => None
-                 | d, m => Some (Node d m I)
-                 end)
-             m2.
-      Definition fold_step elt A
-                 (fold : (list map_key -> elt -> A -> A) -> t elt -> A -> A)
-                 (f : list map_key -> elt -> A -> A)
-                 (m : t elt)
-                 (a : A)
-        : A
-        := t_case_nd
-             (fun d m pf
-              => let a := match d with
-                          | None => a
-                          | Some d => f [] d a
-                          end in
-                 match m with
-                 | Some (exist m pm)
-                   => @map_fold
-                        _ _
-                        (fun k => fold (fun ks => f (k :: ks)))
-                        m
-                        a
-                 | None => a
-                 end)
-             m.
-    End step.
-(*(Node : forall elt (d : option elt) (m : option (map_t_t elt)), node_NonEmpty d m -> t elt)
-              (t_case_nd : forall (elt : Type) (P : Type),
-                  (forall (v : option elt) (m : option (map_t_t elt)), node_NonEmpty v m -> P)
-                  -> t elt -> P)
-              (map_xmap2_l : forall elt elt' elt'', (option elt -> option elt' -> option elt'') -> map_t elt -> map_t elt'')
-              (map_xmap2_r : forall elt elt' elt'', (option elt -> option elt' -> option elt'') -> map_t elt' -> map_t elt'').
-*)
-    Class EverythingGen
-      := { Node : forall elt (d : option elt) (m : option (map_t_t elt)), node_NonEmpty d m -> t elt
-         ; t_case : forall elt (P : t elt -> Type),
-             (forall d m pf, P (@Node elt d m pf))
-             -> forall m, P m
-         ; t_case_beta : forall elt P rec d m pf, @t_case elt P rec (@Node elt d m pf) = rec d m pf
-         ; t_case_nd
-           := fun elt P => @t_case elt (fun _ => P)
-         ; t_ind : forall elt (P : t elt -> Prop),
-             (forall d m pf, (forall k v, @map_find _ k (proj1_sig m) = Some v -> P v) -> P (@Node elt d (Some m) pf))
-             -> forall m, P m
-         ; empty : forall elt, t' elt
-           := fun _ => None
-         ; mapi : forall elt elt', id_fix_2 ((list map_key -> elt -> elt') -> t elt -> t elt')
-         ; mapi_beta : forall elt elt' f m, @mapi elt elt' f m = mapi_step Node t_case_nd (@mapi elt elt') f m
-
-         ; map_xmap2_l : forall elt elt' elt'', (option elt -> option elt' -> option elt'') -> map_t elt -> map_t elt''
-         ; map_xmap2_r : forall elt elt' elt'', (option elt -> option elt' -> option elt'') -> map_t elt' -> map_t elt''
-         ; map_xmap2_lr : forall A B (f g : option A -> option A -> option B) m,
-             (forall i j, f i j = g j i) -> map_xmap2_l f m = map_xmap2_r g m
-         ; map_xgmap2_l : forall A B C (f : option A -> option B -> option C) i m,
-             f None None = None -> @map_find _ i (map_xmap2_l f m) = f (@map_find _ i m) None
-         ; map_xgmap2_r : forall A B C (f : option A -> option B -> option C) i m,
-             f None None = None -> @map_find _ i (map_xmap2_r f m) = f None (@map_find _ i m)
-
-         ; map2_l : forall elt elt' elt'', (option elt -> option elt' -> option elt'') -> id_fix (t elt -> t' elt'')
-         ; map2_r : forall elt elt' elt'', (option elt -> option elt' -> option elt'') -> id_fix (t elt' -> t' elt'')
-         ; map2 : forall elt elt' elt'', (option elt -> option elt' -> option elt'') -> id_fix (t elt -> t elt' -> t' elt'')
-         ; map2_l_beta : forall elt elt' elt'' f m,
-             @map2_l elt elt' elt'' f m = map2_l_step Node t_case_nd map_xmap2_l f (map2_l f) m
-         ; map2_r_beta : forall elt elt' elt'' f m,
-             @map2_r elt elt' elt'' f m = map2_r_step Node t_case_nd map_xmap2_r f (map2_r f) m
-         ; map2_beta : forall elt elt' elt'' f m1 m2,
-             @map2 elt elt' elt'' f m1 m2 = map2_step Node t_case_nd map_xmap2_l map_xmap2_r f (map2_l f) (map2_r f) (map2 f) m1 m2
-         ; fold : forall elt (A : Type), id_fix_2 ((list map_key -> elt -> A -> A) -> t elt -> A -> A)
-         ; fold_beta : forall elt A f m a,
-             @fold elt A f m a = fold_step t_case_nd (@fold elt A) f m a
-      }.
-    Definition Node' {E : EverythingGen} elt (d : option elt) (m : option (map_t_t elt)) : node_NonEmpty' d m -> t elt
-      := match d, m return node_NonEmpty' d m -> _ with
-         | None, None => fun pf => match pf with end
-         | d, (Some _ | None) as m => @Node E elt d m
-         end.
-    Definition oNode_dec_empty {E : EverythingGen} elt (d : option elt) (m : map_t (t elt)) : option (t elt)
-      := match d, dec_empty_cps m (fun x => x) with
-         | None, None => None
-         | d, (None | Some _) as m
-           => Some (Node (d:=d) (m:=m) I)
-         end.
-  End __.
-End EverythingGen.
-Global Arguments Node {t _ _ _ _ _ _ _ _ _ _ _ _} d m _.
-Global Arguments Node' {t _ _ _ _ _ _ _ _ _ _ _ _} d m _.
-
-Create HintDb trie_db discriminated.
-
-Hint Rewrite
-     t_case_beta
-     mapi_beta
-     map2_beta
-     map2_l_beta
-     map2_r_beta
-     fold_beta
-  : trie_db.
-
-Hint Unfold
-     id_fix
-     id_fix_2
-     id_case
-     Node'
-     oNode_dec_empty
-     empty'
-     mapi_step
-     map2_step
-     map2_l_step
-     map2_r_step
-     fold_step
-     t_case_nd
-     empty
-  : trie_db.
-
-Module Type MapEmptyTyp (label : DecidableType) (map : FMapInterface.WSfun label).
-  Parameter map_NonEmpty : forall elt, map.t elt -> Prop.
-  Axiom map_NonEmpty_iff : forall elt m, @map_NonEmpty elt m <-> ~map.Empty m.
-End MapEmptyTyp.
-
-Module InnerTrieShape (label : DecidableType) (map : FMapInterface.WSfun label) (Import T : TypFunctor) (Import ME : MapEmptyTyp label map).
-  Lemma map_mapi_nonEmpty : forall elt elt' f m, @map_NonEmpty _ m -> @map_NonEmpty _ (@map.mapi elt elt' f m).
-  Proof.
-    intros *; rewrite !map_NonEmpty_iff.
-    cbv [map.Empty]; intros H H'; apply H; clear H.
-    intros k v H; specialize (H' k).
-    eapply map.mapi_1 in H.
-    destruct H as [? [? H]].
-    apply H' in H.
-    exact H.
-  Qed.
-  Lemma map_is_empty_1 : forall elt m, @map.is_empty elt m = false -> @map_NonEmpty elt m.
-  Proof.
-    intros *; rewrite !map_NonEmpty_iff; intros H H'; apply map.is_empty_1 in H'; congruence.
-  Qed.
-End InnerTrieShape.
-Module Type TrieShape (label : DecidableType) (map : FMapInterface.WSfun label) (Import T : TypFunctor) (Import ME : MapEmptyTyp label map).
-  Module Import _TrieShape := InnerTrieShape label map T ME.
-  Notation Everything := (@EverythingGen t map.key map.t map.is_empty map_NonEmpty map_is_empty_1 map.fold map.mapi map_mapi_nonEmpty map.map2 map.find).
-End TrieShape.
-
-Module Type Trie (label : DecidableType) (map : FMapInterface.WSfun label).
-  Parameter t : Type -> Type.
-  Include MapEmptyTyp label map.
-  Include TrieShape label map.
-  Parameter Inline everything : Everything.
-  Existing Instance everything.
-End Trie.
-
-Local Ltac t_destr_conj_step :=
-  first [ progress subst
-        | progress destruct_head'_False
-        | progress destruct_head'_and
-        | progress destruct_head'_ex
-        | progress destruct_head'_True
-        | progress destruct_head'_unit
-        | progress destruct_head' sig
-        | progress inversion_option
-        | progress inversion_sigma
-        | progress inversion_list
-        | progress inversion_pair
-        | progress cbn [fst snd proj1_sig proj2_sig] in *
-        | match goal with
-          | [ H : eqlistA _ nil _ |- _ ] => inversion H; clear H
-          | [ H : eqlistA _ _ nil |- _ ] => inversion H; clear H
-          | [ H : eqlistA _ (_ :: _) _ |- _ ] => inversion H; clear H
-          | [ H : eqlistA _ _ (_ :: _) |- _ ] => inversion H; clear H
-          | [ H : InA _ _ (_ :: _) |- _ ] => inversion H; clear H
-          | [ H : InA _ _ nil |- _ ] => inversion H; clear H
-          | [ H : List.In _ (List.map _ _) |- _ ] => rewrite in_map_iff in H
-          | [ H : List.In _ (List.flat_map _ _) |- _ ] => rewrite in_flat_map in H
-          | [ H : ?x = ?x |- _ ] => clear H
-          | [ H : ?T, H' : ?T |- _ ] => clear H
-          | [ H : ?x = Some _, H' : context[?x] |- _ ] => rewrite H in H'
-          | [ H : ?x = None, H' : context[?x] |- _ ] => rewrite H in H'
-          | [ H : Some _ = ?x |- _ ] => symmetry in H
-          | [ H : None = ?x |- _ ] => symmetry in H
-          end
-        | discriminate ].
-Local Ltac t_destr_step :=
-  first [ t_destr_conj_step
-        | progress destruct_head'_or
-        | progress destruct_head' option
-        | break_innermost_match_hyps_step
-        | break_innermost_match_step ].
-Local Ltac t_specialize_safe_step :=
-  first [ progress specialize_by_assumption
-        | progress cbv [not] in *
-        | progress specialize_by reflexivity
-        | progress specialize_under_binders_by apply conj
-        | progress specialize_under_binders_by eapply ex_intro
-        | progress specialize_under_binders_by apply eqlistA_cons ].
 
 Module ListWSfun_gen (Y : DecidableTypeOrig) (M : WSfun Y) (Import T : Trie Y M).
   Module Type ESig := ListTyp Y <+ HasEq <+ IsEqOrig <+ HasEqDec.
@@ -431,9 +68,10 @@ Module ListWSfun_gen (Y : DecidableTypeOrig) (M : WSfun Y) (Import T : Trie Y M)
 
     Global Hint Transparent key : core.
 
-    Definition t elt := option (T.t elt).
-
-    Hint Rewrite map_NonEmpty_iff : trie_db.
+    Notation t' elt := (option (T.t elt)).
+    Notation t'_P m := (True -> match m with None => True | Some m' => recursively_non_empty m' = true end) (only parsing).
+    Notation mk m pf := (exist (fun m' => t'_P m') m (fun 'I => pf)).
+    Definition t elt := { m : t' elt | t'_P m }.
 
     Local Ltac t_obgl :=
       repeat first [ progress intros
@@ -461,12 +99,9 @@ Module ListWSfun_gen (Y : DecidableTypeOrig) (M : WSfun Y) (Import T : Trie Y M)
                    | progress subst
                    | progress specialize_under_binders_by eapply M.map_1
                    | progress break_innermost_match_hyps
-                   | rewrite map_NonEmpty_iff in *
                    | progress specialize_under_binders_by (match goal with |- M.MapsTo _ _ (M.map2 _ _ _) => idtac end;
                                                            eapply M.find_2;
                                                            rewrite M.map2_1) ].
-
-    Local Obligation Tactic := (*try abstract t_obgl;*) t_obgl.
 
     Local Ltac pose_MapsTo_as_find lem :=
       let H := fresh in
@@ -486,7 +121,7 @@ Module ListWSfun_gen (Y : DecidableTypeOrig) (M : WSfun Y) (Import T : Trie Y M)
       induction m as [d m pf IH] using (t_ind (elt:=elt)); intros.
       repeat (autounfold with trie_db; autorewrite with trie_db).
       clear pf.
-      destruct m as [m pf]; cbn [proj1_sig] in *; clear pf.
+      break_innermost_match_hyps; try now break_innermost_match; eauto.
       rewrite !M.fold_1.
       erewrite fold_left_ext_in; [ f_equal; try reflexivity; break_innermost_match; eauto | ].
       intros.
@@ -501,159 +136,6 @@ Module ListWSfun_gen (Y : DecidableTypeOrig) (M : WSfun Y) (Import T : Trie Y M)
     Proof.
       intros f g Hfg; repeat intro; eapply fold_ext; cbv in *; eauto.
     Qed.
-
-    Section Types.
-      Variable elt:Type.
-      Definition empty : t elt := None.
-      Definition is_empty : t elt -> bool := Option.is_None.
-      Program Fixpoint add' (x : key) (y : elt) (m : t elt) {struct x} : T.t elt
-        := match x return _ with
-           | []
-             => Node (Some y) (m <- m; t_case_nd (fun _ m _ => m) m) I
-           | x :: xs
-             => let default d := Node' d (Some (exist _ (M.add x (add' xs y empty) (@M.empty _)) _)) I in
-                match m return _ with
-                | None
-                  => default None
-                | Some m
-                  => t_case_nd
-                       (fun d m pf
-                        => match m return _ with
-                           | None => default d
-                           | Some (exist m pf)
-                             => let m' := M.find x m in
-                                Node'
-                                  d
-                                  (Some
-                                     (exist
-                                        _
-                                        (M.add x (add' xs y m') m)
-                                        _))
-                                  I
-                           end)
-                       m
-                end
-           end.
-      Definition add (x : key) (y : elt) (m : t elt) : t elt
-        := Some (add' x y m).
-      Fixpoint find (x : key) (m : t elt) {struct x} : option elt
-        := (m <- m;
-            match x with
-            | [] => t_case_nd (fun v _ _ => v) m
-            | x :: xs
-              => t_case_nd
-                   (fun v m pf
-                    => match m with
-                       | Some (exist m mp) => find xs (M.find x m)
-                       | None => None
-                       end)
-                   m
-            end).
-      Program Fixpoint remove (k : key) (m : t elt) : t elt
-        := (m <- m;
-            match k return _ with
-            | []
-              => t_case_nd
-                   (fun d m pf
-                    => match m return _ with
-                       | None => None
-                       | Some m => Some (Node' None (Some m) I)
-                       end)
-                   m
-            | x :: xs
-              => t_case_nd
-                   (fun d m pf
-                    => let default : t elt := Some (Node d m pf) in
-                       match m return _ with
-                       | None => default
-                       | Some (exist m mp)
-                         => match remove xs (M.find x m) return _ with
-                            | None
-                              => oNode_dec_empty d (M.remove x m)
-                            | Some m'
-                              => Some (Node' d (Some (exist _ (M.add x m' m) _)) I)
-                            end
-                       end)
-                   m
-            end).
-      Definition mem (x : key) (m : t elt) : bool := Option.is_Some (find x m).
-      Variable elt' elt'' : Type.
-
-      Definition mapi (f : key -> elt -> elt') : t elt -> t elt'
-        := option_map (mapi f).
-      Definition map (f : elt -> elt') : t elt -> t elt' := mapi (fun _ => f).
-      Definition map2 (f : option elt -> option elt' -> option elt'') (m1 : t elt) (m2 : t elt') : t elt''
-        := match m1, m2 with
-           | None, None => None
-           | Some m1, Some m2 => map2 f m1 m2
-           | Some m1, None => map2_l f m1
-           | None, Some m2 => map2_r f m2
-           end.
-      Definition fold A (f : key -> elt -> A -> A) (m : t elt) (a : A) : A
-        := match m with
-           | None => a
-           | Some m => fold f m a
-           end.
-      Definition elements_with_key_prefix_and (m : t elt) (k_prefix : key) prefix : list (key*elt)
-        := List.rev_append (fold (fun k v rest => (k_prefix ++ k, v) :: rest) m prefix) nil.
-      Definition elements (m : t elt) : list (key*elt) := elements_with_key_prefix_and m nil nil.
-      Definition cardinal (m : t elt) : nat := List.length (elements m).
-    End Types.
-
-    Definition equal elt (cmp : elt -> elt -> bool) (m1 m2 : t elt) : bool
-      := let cmp' x y
-           := match x, y with
-              | Some x, Some y => Some (cmp x y)
-              | Some _, None
-              | None, Some _
-                => Some false
-              | None, None => None
-              end in
-         fold (fun _ => andb) (map2 cmp' m1 m2) true.
-    Definition MapsTo elt (k : key) (v : elt) (m : t elt) : Prop
-      := find k m = Some v.
-    Definition eq_key elt (p p':key*elt) := E.eq (fst p) (fst p').
-    Definition eq_key_elt elt (p p':key*elt) :=
-      E.eq (fst p) (fst p') /\ (snd p) = (snd p').
-
-    Local Instance Proper_M_eq_key_elt_iff elt
-      : Proper (eq ==> RelationPairs.RelProd Y.eq eq ==> iff) (@M.eq_key_elt elt).
-    Proof. cbv; repeat intro; subst; destruct_head'_prod; destruct_head'_and; subst; firstorder (subst; eauto). Qed.
-
-    Local Instance Proper_M_eq_key_elt_impl elt
-      : Proper (eq ==> RelationPairs.RelProd Y.eq eq ==> impl) (@M.eq_key_elt elt).
-    Proof. cbv; repeat intro; subst; destruct_head'_prod; destruct_head'_and; subst; firstorder (subst; eauto). Qed.
-
-    Local Instance Proper_M_eq_key_elt_flip_impl elt
-      : Proper (eq ==> RelationPairs.RelProd Y.eq eq ==> flip impl) (@M.eq_key_elt elt).
-    Proof. cbv; repeat intro; subst; destruct_head'_prod; destruct_head'_and; subst; firstorder (subst; eauto). Qed.
-
-    Local Instance Proper_M_eq_key_elt_iff' elt
-      : Proper (@M.eq_key_elt elt ==> @M.eq_key_elt elt ==> iff) (@M.eq_key_elt elt).
-    Proof. cbv; repeat intro; subst; destruct_head'_prod; destruct_head'_and; subst; firstorder (subst; eauto). Qed.
-
-    Local Instance Proper_M_eq_key_elt_impl' elt
-      : Proper (@M.eq_key_elt elt ==> @M.eq_key_elt elt ==> impl) (@M.eq_key_elt elt).
-    Proof. cbv; repeat intro; subst; destruct_head'_prod; destruct_head'_and; subst; firstorder (subst; eauto). Qed.
-
-    Local Instance Proper_M_eq_key_elt_flip_impl' elt
-      : Proper (@M.eq_key_elt elt ==> @M.eq_key_elt elt ==> flip impl) (@M.eq_key_elt elt).
-    Proof. cbv; repeat intro; subst; destruct_head'_prod; destruct_head'_and; subst; firstorder (subst; eauto). Qed.
-
-    Local Instance Proper_M_eq_key_iff elt
-      : Proper (@M.eq_key elt ==> @M.eq_key elt ==> iff) (@M.eq_key elt).
-    Proof. cbv; repeat intro; subst; destruct_head'_prod; destruct_head'_and; subst; firstorder (subst; eauto). Qed.
-
-    Local Instance Proper_M_eq_key_impl elt
-      : Proper (@M.eq_key elt ==> @M.eq_key elt ==> impl) (@M.eq_key elt).
-    Proof. cbv; repeat intro; subst; destruct_head'_prod; destruct_head'_and; subst; firstorder (subst; eauto). Qed.
-
-    Local Instance Proper_M_eq_key_flip_impl elt
-      : Proper (@M.eq_key elt ==> @M.eq_key elt ==> flip impl) (@M.eq_key elt).
-    Proof. cbv; repeat intro; subst; destruct_head'_prod; destruct_head'_and; subst; firstorder (subst; eauto). Qed.
-
-    Local Instance M_Equal_Equivalence elt : Equivalence (@M.Equal elt) | 10.
-    Proof. split; cbv; firstorder eauto using eq_trans. Qed.
 
     Hint Extern 1 (ProperProxy (@M.Equal _) _) => apply reflexive_proper_proxy : typeclass_instances.
 
@@ -694,23 +176,47 @@ Module ListWSfun_gen (Y : DecidableTypeOrig) (M : WSfun Y) (Import T : Trie Y M)
     Local Instance M_In_compat elt : Proper (Y.eq ==> @M.Equal _ ==> iff) (@M.In elt) | 10.
     Proof. t_Proper_helper. Qed.
 
-    Local Instance eq_key_equiv elt : Equivalence (@eq_key elt) | 10.
-    Proof.
-      split; cbv; intros; break_innermost_match; break_innermost_match_hyps; try ((idtac + symmetry + etransitivity + exfalso); (eassumption + reflexivity)).
-    Qed.
-    Local Instance eq_key_elt_equiv elt : Equivalence (@eq_key_elt elt) | 10.
-    Proof.
-      split; cbv; intros; break_innermost_match; break_innermost_match_hyps; destruct_head'_and; split; try ((idtac + symmetry + etransitivity + exfalso); (eassumption + reflexivity)).
-    Qed.
+    Local Instance Proper_M_eq_key_elt_iff elt
+      : Proper (eq ==> RelationPairs.RelProd Y.eq eq ==> iff) (@M.eq_key_elt elt).
+    Proof. cbv; repeat intro; subst; destruct_head'_prod; destruct_head'_and; subst; firstorder (subst; eauto). Qed.
 
-    Definition In elt (k : key) (m : t elt) := exists e, MapsTo k e m.
-    Definition Empty elt (m : t elt) := forall a e, ~ MapsTo a e m.
-    Definition Equal elt (m m' : t elt) := forall y, find y m = find y m'.
-    Definition Equiv elt (eq_elt:elt->elt->Prop) m m' :=
-      (forall k, In k m <-> In k m') /\
-        (forall k e e', MapsTo k e m -> MapsTo k e' m' -> eq_elt e e').
-    Definition Equivb elt (cmp: elt->elt->bool) := Equiv (Cmp cmp).
+    Local Instance Proper_M_eq_key_elt_impl elt
+      : Proper (eq ==> RelationPairs.RelProd Y.eq eq ==> impl) (@M.eq_key_elt elt).
+    Proof. cbv; repeat intro; subst; destruct_head'_prod; destruct_head'_and; subst; firstorder (subst; eauto). Qed.
 
+    Local Instance Proper_M_eq_key_elt_flip_impl elt
+      : Proper (eq ==> RelationPairs.RelProd Y.eq eq ==> flip impl) (@M.eq_key_elt elt).
+    Proof. cbv; repeat intro; subst; destruct_head'_prod; destruct_head'_and; subst; firstorder (subst; eauto). Qed.
+
+    Local Instance Proper_M_eq_key_elt_iff' elt
+      : Proper (@M.eq_key_elt elt ==> @M.eq_key_elt elt ==> iff) (@M.eq_key_elt elt).
+    Proof. cbv; repeat intro; subst; destruct_head'_prod; destruct_head'_and; subst; firstorder (subst; eauto). Qed.
+
+    Local Instance Proper_M_eq_key_elt_impl' elt
+      : Proper (@M.eq_key_elt elt ==> @M.eq_key_elt elt ==> impl) (@M.eq_key_elt elt).
+    Proof. cbv; repeat intro; subst; destruct_head'_prod; destruct_head'_and; subst; firstorder (subst; eauto). Qed.
+
+    Local Instance Proper_M_eq_key_elt_flip_impl' elt
+      : Proper (@M.eq_key_elt elt ==> @M.eq_key_elt elt ==> flip impl) (@M.eq_key_elt elt).
+    Proof. cbv; repeat intro; subst; destruct_head'_prod; destruct_head'_and; subst; firstorder (subst; eauto). Qed.
+
+    Local Instance Proper_M_eq_key_iff elt
+      : Proper (@M.eq_key elt ==> @M.eq_key elt ==> iff) (@M.eq_key elt).
+    Proof. cbv; repeat intro; subst; destruct_head'_prod; destruct_head'_and; subst; firstorder (subst; eauto). Qed.
+
+    Local Instance Proper_M_eq_key_impl elt
+      : Proper (@M.eq_key elt ==> @M.eq_key elt ==> impl) (@M.eq_key elt).
+    Proof. cbv; repeat intro; subst; destruct_head'_prod; destruct_head'_and; subst; firstorder (subst; eauto). Qed.
+
+    Local Instance Proper_M_eq_key_flip_impl elt
+      : Proper (@M.eq_key elt ==> @M.eq_key elt ==> flip impl) (@M.eq_key elt).
+    Proof. cbv; repeat intro; subst; destruct_head'_prod; destruct_head'_and; subst; firstorder (subst; eauto). Qed.
+
+    Local Instance M_Equal_Equivalence elt : Equivalence (@M.Equal elt) | 10.
+    Proof. split; cbv; firstorder eauto using eq_trans. Qed.
+
+    Lemma M_is_empty_iff elt (m : M.t elt) : M.is_empty m = true <-> M.Empty m.
+    Proof. split; first [ apply M.is_empty_1 | apply M.is_empty_2 ]. Qed.
     Lemma M_find_iff elt m x e : @M.MapsTo elt x e m <-> M.find x m = Some e.
     Proof. split; first [ apply M.find_1 | apply M.find_2 ]. Qed.
     Lemma M_find_empty elt x : M.find x (@M.empty elt) = None.
@@ -719,6 +225,476 @@ Module ListWSfun_gen (Y : DecidableTypeOrig) (M : WSfun Y) (Import T : Trie Y M)
       cbv in H; setoid_rewrite M_find_iff in H.
       destruct M.find; intuition congruence.
     Qed.
+
+    Local Ltac Proper_equiv_t :=
+      cbv;
+      setoid_rewrite M_find_iff;
+      repeat split; intros; subst; split_and; eauto.
+
+    Local Instance Proper_M_Equiv_eq_impl elt
+      : Proper ((eq ==> eq ==> impl) ==> eq ==> eq ==> impl) (@M.Equiv elt) | 10.
+    Proof. Proper_equiv_t. Qed.
+    Local Instance Proper_M_Equiv_eq_flip_impl elt
+      : Proper ((eq ==> eq ==> flip impl) ==> eq ==> eq ==> flip impl) (@M.Equiv elt) | 10.
+    Proof. Proper_equiv_t. Qed.
+    Local Instance Proper_M_Equiv_eq_iff elt
+      : Proper ((eq ==> eq ==> iff) ==> eq ==> eq ==> iff) (@M.Equiv elt) | 10.
+    Proof. Proper_equiv_t. Qed.
+    Local Instance Proper_M_Equiv_eq_impl_pointwise elt
+      : Proper (pointwise_relation _ (pointwise_relation _ impl) ==> eq ==> eq ==> impl) (@M.Equiv elt) | 10.
+    Proof. Proper_equiv_t. Qed.
+    Local Instance Proper_M_Equiv_eq_flip_impl_pointwise elt
+      : Proper (pointwise_relation _ (pointwise_relation _ (flip impl)) ==> eq ==> eq ==> flip impl) (@M.Equiv elt) | 10.
+    Proof. Proper_equiv_t. Qed.
+    Local Instance Proper_M_Equiv_eq_iff_pointwise elt
+      : Proper (pointwise_relation _ (pointwise_relation _ iff) ==> eq ==> eq ==> iff) (@M.Equiv elt) | 10.
+    Proof. Proper_equiv_t. Qed.
+
+
+    Lemma M_elements_iff elt m x e
+      : M.MapsTo x e m <-> InA (M.eq_key_elt (elt:=elt)) (x, e) (M.elements m).
+    Proof. split; first [ apply M.elements_1 | apply M.elements_2 ]. Qed.
+    Lemma M_forall_In_elements_iff elt (P : _ -> Prop) (m : M.t elt)
+          (P_Proper : Proper (@M.eq_key_elt _ ==> Basics.flip impl) P)
+      : (forall i, List.In i (M.elements m) -> P i)
+        <-> (forall k v, M.find k m = Some v -> P (k, v)).
+    Proof.
+      setoid_rewrite <- M_find_iff.
+      setoid_rewrite M_elements_iff.
+      setoid_rewrite InA_alt.
+      split; intros; destruct_head' prod; repeat t_destr_step; firstorder eauto.
+    Qed.
+    Lemma M_forall_In_elements_snd_iff elt (P : _ -> Prop) (m : M.t elt)
+      : (forall i, List.In i (M.elements m) -> P (snd i))
+        <-> (forall k v, M.find k m = Some v -> P v).
+    Proof.
+      rewrite M_forall_In_elements_iff; [ reflexivity | ].
+      cbv; repeat intro; repeat t_destr_step; assumption.
+    Qed.
+
+    Lemma M_add_full elt0 m0 v x' y' : @M.find elt0 y' (M.add x' v m0) = if Y.eq_dec x' y' then Some v else M.find y' m0.
+    Proof using Type.
+      clear.
+      pose_MapsTo_as_find M.add_1.
+      pose_MapsTo_as_find M.add_2.
+      pose_MapsTo_as_find M.add_3.
+      repeat match goal with
+             | [ |- context[M.find ?x ?m] ]
+               => destruct (M.find x m) eqn:?
+             end.
+      all: break_innermost_match.
+      all: specialize_under_binders_by eassumption.
+      all: intuition congruence.
+    Qed.
+    Hint Rewrite M_add_full : list_map_alt.
+    Local Ltac t_full_step :=
+      first [ t_destr_step
+            | progress cbv [M.In not option_map] in *
+            | progress intros
+            | match goal with
+              | [ H : context[M.MapsTo] |- _ ] => setoid_rewrite M_find_iff in H
+              | [ |- context[M.MapsTo] ] => setoid_rewrite M_find_iff
+              end
+            | progress specialize_under_binders_by eapply ex_intro
+            | progress specialize_under_binders_by eassumption
+            | progress specialize_under_binders_by reflexivity
+            | exfalso; assumption
+            | progress inversion_option
+            | progress subst
+            | reflexivity
+            | break_innermost_match_step
+            | match goal with
+              | [ |- context[M.find ?x ?y] ] => destruct (M.find x y) eqn:?
+              end ].
+
+    Lemma M_remove_full elt0 m0 x' y' : @M.find elt0 y' (M.remove x' m0) = if Y.eq_dec x' y' then None else M.find y' m0.
+    Proof using Type.
+      clear.
+      pose proof (@M.remove_1 elt0 m0 x' y') as H0.
+      pose_MapsTo_as_find (@M.remove_2 elt0 m0 x' y').
+      pose_MapsTo_as_find (@M.remove_3 elt0 m0 x' y').
+      repeat t_full_step.
+    Qed.
+    Hint Rewrite M_remove_full : list_map_alt.
+
+    Lemma M_mapi_full : forall (elt elt':Type)(m: M.t elt)(x:M.key)(f:M.key->elt->elt'), exists y, Y.eq y x /\ M.find x (M.mapi f m) = option_map (f y) (M.find x m).
+    Proof.
+      pose proof M.mapi_1 as H.
+      pose proof M.mapi_2 as H'.
+      repeat t_full_step.
+      all: match goal with
+           | [ H : M.find _ (M.mapi _ _) = _ |- _ ]
+             => in_hyp_under_binders_do (fun H' => rewrite H in H')
+           end.
+      all: repeat t_full_step; eauto.
+    Qed.
+    Hint Rewrite M_mapi_full : list_map_alt.
+    Lemma M_mapi_full_impl (elt elt':Type)(m: M.t elt)(f:M.key->elt->elt')(P:_->Prop)
+      : (forall x e, M.find x (M.mapi f m) = Some e -> P e)
+        -> (forall x, exists y, Y.eq y x /\ forall e, option_map (f y) (M.find x m) = Some e -> P e).
+    Proof.
+      intros H x.
+      specialize (H x).
+      destruct (@M_mapi_full _ _ m x f) as [? [H0 H1]].
+      eexists; split; [ eassumption | ].
+      specialize_under_binders_by rewrite H1.
+      intuition congruence.
+    Qed.
+    Lemma M_map2_full
+      : forall (elt elt' elt'':Type)(m: M.t elt)(m': M.t elt')
+	       (x:M.key)(f:option elt->option elt'->option elt''),
+        M.find x (M.map2 f m m') = match M.find x m, M.find x m' with
+                                   | None, None => None
+                                   | x, y => f x y
+                                   end.
+    Proof.
+      intros *.
+      pose proof (@M.map2_1 elt elt' elt'' m m' x f) as H.
+      pose proof (@M.map2_2 elt elt' elt'' m m' x f) as H'.
+      cbv [M.In] in *.
+      setoid_rewrite M_find_iff in H.
+      setoid_rewrite M_find_iff in H'.
+      specialize_under_binders_by eapply ex_intro.
+      destruct (M.find x (M.map2 f m m')); break_innermost_match; try reflexivity;
+        specialize_by eauto; specialize_under_binders_by reflexivity; eauto.
+      firstorder congruence.
+    Qed.
+    Hint Rewrite M_map2_full : list_map_alt.
+
+    Create HintDb list_map_non_empty_db discriminated.
+
+    Local Ltac t_non_empty_handle_add_step :=
+      first [ match goal with
+              | [ H : context[M.find _ (M.add _ _ _)] |- _ ]
+                => setoid_rewrite M_add_full in H
+              | [ |- context[M.find _ (M.add _ _ _)] ]
+                => setoid_rewrite M_add_full
+              | [ H : forall k v, (if Y.eq_dec ?x k then @?A k v else @?B k v) = Some v -> @?P k v |- _ ]
+                => assert (forall v, A x v = Some v -> P x v)
+                  by (let v := fresh in
+                      intros v;
+                      specialize (H x v);
+                      destruct (Y.eq_dec x x);
+                      [ exact H | now exfalso; eauto ]);
+                   assert (forall k v, (Y.eq x k -> False) -> B k v = Some v -> False)
+                     by (let k := fresh in
+                         let v := fresh in
+                         let H' := fresh in
+                         intros k v H';
+                         specialize (H k v);
+                         destruct (Y.eq_dec x k);
+                         [ now exfalso; eauto | exact H ]);
+                   clear H
+              end ].
+    Local Ltac t_non_empty_handle_remove_step :=
+      first [ match goal with
+              | [ H : context[M.find _ (M.remove _ _)] |- _ ]
+                => setoid_rewrite M_remove_full in H
+              | [ |- context[M.find _ (M.remove _ _)] ]
+                => setoid_rewrite M_remove_full
+              end ].
+    Local Ltac t_non_empty_handle_mapi_step :=
+      first [ match goal with
+              | [ H : context[M.find _ (M.mapi _ _)] |- _ ]
+                => setoid_rewrite M_mapi_full in H
+              | [ |- context[M.find _ (M.mapi _ _)] ]
+                => setoid_rewrite M_mapi_full
+              | [ H : context[M.find ?k (M.mapi ?f ?m)] |- _ ]
+                => let H' := fresh in
+                   destruct (@M_mapi_full _ _ m k f) as [? [? H']];
+                   rewrite H' in H; rewrite ?H' in *; clear H'; cbv [option_map] in *
+              | [ |- context[M.find ?k (M.mapi ?f ?m)] ]
+                => let H' := fresh in
+                   destruct (@M_mapi_full _ _ m k f) as [? [? H']];
+                   rewrite H'; rewrite ?H' in *; clear H'; cbv [option_map] in *
+              | [ H : forall x e, M.find x (M.mapi ?f ?m) = Some e -> @?P e |- _ ]
+                => pose proof (@M_mapi_full_impl _ _ m f P H);
+                   clear H
+              end ].
+    Local Ltac t_non_empty_handle_map2_step :=
+      first [ match goal with
+              | [ H : context[M.find _ (M.map2 _ _ _)] |- _ ]
+                => setoid_rewrite M_map2_full in H
+              | [ |- context[M.find _ (M.map2 _ _ _)] ]
+                => setoid_rewrite M_map2_full
+              | [ H : context[M.find _ (map_xmap2_l _ _)] |- _ ]
+                => setoid_rewrite map_xgmap2_l in H; [ | reflexivity ]
+              | [ H : context[M.find _ (map_xmap2_r _ _)] |- _ ]
+                => setoid_rewrite map_xgmap2_r in H; [ | reflexivity ]
+              end ].
+    Local Ltac t_non_empty_extra_step :=
+      first [ match goal with
+              | [ H : forall k v, M.find k ?m = Some v -> ?f v = true, H' : forall k' v', M.find k' ?m = Some v' -> ?f v' = true -> _ |- _ ]
+                => specialize (fun k' v' pf => H' k' v' pf (H _ _ pf))
+              | [ H : forall k v, M.find k ?m = Some v -> ?f v = true, H' : forall k' v', M.find k' ?m = Some v' -> _ -> ?f v' = true -> _ |- _ ]
+                => specialize (fun k' v' pf pf' => H' k' v' pf pf' (H _ _ pf))
+              end ].
+
+    Local Ltac t_non_empty_step :=
+      first [ t_destr_conj_step
+            | assumption
+            | reflexivity
+            | progress specialize_under_binders_by exact I
+            | progress intros
+            | rewrite M.fold_1 in *
+            | rewrite <- (fun c => @fold_left_map _ _ c andb), @fold_left_andb_truth_map_iff in *
+            | rewrite negb_true_iff, <- not_true_iff_false in *
+            | rewrite M_is_empty_iff in *
+            | rewrite M_find_empty in *
+            | t_destr_step
+            | progress cbv [M.Empty not] in *
+            | progress cbn [option_map Option.bind] in *
+            | progress specialize_under_binders_by (idtac; lazymatch goal with |- True -> _ => idtac end;
+                                                    intros _)
+            | match goal with
+              | [ H : forall x, Some ?y = Some x -> _ |- _ ]
+                => specialize (H y eq_refl)
+              | [ H : context[M.MapsTo] |- _ ] => setoid_rewrite M_find_iff in H
+              | [ |- context[M.MapsTo] ] => setoid_rewrite M_find_iff
+              | [ H : context[forall i, List.In i (M.elements _) -> ?f (snd i) = true] |- _ ]
+                => setoid_rewrite M_forall_In_elements_snd_iff with (P:=fun e => f e = true) in H
+              | [ |- context[forall i, List.In i (M.elements _) -> ?f (snd i) = true] ]
+                => setoid_rewrite M_forall_In_elements_snd_iff with (P:=fun e => f e = true)
+              end
+            | t_non_empty_handle_add_step
+            | t_non_empty_handle_remove_step
+            | t_non_empty_handle_map2_step
+            | t_non_empty_handle_mapi_step
+            | t_non_empty_extra_step
+            | match goal with
+              | [ |- _ /\ _ ] => split
+              end
+            | solve [ eauto with nocore ] ].
+
+    Section Types.
+      Variable elt:Type.
+      Definition empty : t elt := mk None I.
+      Definition is_empty (m : t elt) : bool := Option.is_None (proj1_sig m).
+      Fixpoint add' (x : key) (y : elt) (m : t' elt) {struct x} : T.t elt
+        := match x return T.t elt with
+           | []
+             => Node (Some y) (m <- m; t_case_nd (fun _ m _ => m) m) I
+           | x :: xs
+             => let add_to d m' m := Node' d (Some (M.add x (add' xs y m') m)) I in
+                let default d := add_to d None (@M.empty _) in
+                match m return T.t elt with
+                | None
+                  => default None
+                | Some m
+                  => t_case_nd
+                       (fun d m pf
+                        => match m return T.t elt with
+                           | None => default d
+                           | Some m
+                             => add_to d (M.find x m) m
+                           end)
+                       m
+                end
+           end.
+      Lemma add_non_empty x y m (pf : t'_P m) : t'_P (Some (add' x y m)).
+      Proof using Type.
+        intros _; specialize (pf I); cbv beta iota.
+        revert m pf.
+        induction x as [|x xs IH], m as [m|];
+          try (induction m as [d m] using (t_case (elt:=elt)));
+          cbn [add' Option.bind];
+          repeat (break_innermost_match; autounfold with trie_db; autorewrite with trie_db).
+        all: repeat t_non_empty_step.
+        all: solve [ apply IH; clear IH; repeat t_non_empty_step ].
+      Qed.
+      Definition add (x : key) (y : elt) (m : t elt) : t elt
+        := mk (Some (add' x y (proj1_sig m))) (add_non_empty x y (proj2_sig m) I).
+      Fixpoint find' (x : key) (m : t' elt) {struct x} : option elt
+        := (m <- m;
+            match x with
+            | [] => t_case_nd (fun v _ _ => v) m
+            | x :: xs
+              => t_case_nd
+                   (fun v m pf => m <- m; find' xs (M.find x m))
+                   m
+            end).
+      Definition find (x : key) (m : t elt) : option elt
+        := find' x (proj1_sig m).
+      Fixpoint remove' (k : key) (m : t' elt) {struct k} : t' elt
+        := (m <- m;
+            match k return _ with
+            | []
+              => t_case_nd
+                   (fun d m pf
+                    => match m return _ with
+                       | None => None
+                       | Some m => Some (Node' None (Some m) I)
+                       end)
+                   m
+            | x :: xs
+              => t_case_nd
+                   (fun d m pf
+                    => let default : t' elt := Some (Node d m pf) in
+                       match m return _ with
+                       | None => default
+                       | Some m
+                         => match remove' xs (M.find x m) return _ with
+                            | None
+                              => oNode_dec_empty d (M.remove x m)
+                            | Some m'
+                              => Some (Node' d (Some (M.add x m' m)) I)
+                            end
+                       end)
+                   m
+            end).
+      Lemma remove_non_empty x m (pf : t'_P m) : t'_P (remove' x m).
+      Proof using Type.
+        intros _; specialize (pf I); cbv beta iota.
+        destruct (remove' x m) as [m'|] eqn:H; [ | exact I ].
+        revert m m' H pf.
+        induction x as [|x xs IH], m as [m|];
+          try (induction m as [d m] using (t_case (elt:=elt)));
+          cbn [remove' Option.bind];
+          intros *;
+          repeat match goal with
+                 | [ |- Some _ = Some _ -> _ ] => intro; inversion_option; subst
+                 | [ |- None = Some _ -> _ ] => intro; inversion_option; subst
+                 | _ => break_innermost_match; autounfold with trie_db; autorewrite with trie_db
+                 end.
+        all: repeat t_non_empty_step.
+        all: solve [ eapply IH; [ eassumption | ]; clear IH; repeat t_non_empty_step ].
+      Qed.
+      Definition remove (x : key) (m : t elt) : t elt
+        := mk (remove' x (proj1_sig m)) (remove_non_empty x (proj2_sig m) I).
+      Definition mem (x : key) (m : t elt) : bool := Option.is_Some (find x m).
+      Variable elt' elt'' : Type.
+      Lemma mapi_non_empty (f : key -> elt -> elt') (m : t' elt) (pf : t'_P m) : t'_P (option_map (mapi f) m).
+      Proof using Type.
+        clear -pf.
+        intros _; specialize (pf I); cbv beta iota.
+        destruct m as [m|]; cbv [option_map]; [ | exact I ].
+        revert f pf.
+        induction m as [d m pf IH] using (t_ind (elt:=elt)); intro f;
+          repeat (autounfold with trie_db; autorewrite with trie_db).
+        all: repeat t_non_empty_step.
+        all: repeat match goal with
+                    | [ H : context[recursively_non_empty] |- _ ] => clear H
+                    end.
+        all: exactly_once (idtac; multimatch goal with
+                                  | [ H : ?T -> False |- False ]
+                                    => apply H; clear H
+                                  end).
+        all: intros; specialize_all_ways.
+        all: repeat t_non_empty_step.
+      Qed.
+      Definition mapi (f : key -> elt -> elt') (m : t elt) : t elt'
+        := mk (option_map (mapi f) (proj1_sig m)) (mapi_non_empty f (proj2_sig m) I).
+      Definition map (f : elt -> elt') : t elt -> t elt' := mapi (fun _ => f).
+      Definition map2' (f : option elt -> option elt' -> option elt'') (m1 : t' elt) (m2 : t' elt') : t' elt''
+        := match m1, m2 with
+           | None, None => None
+           | Some m1, Some m2 => map2 f m1 m2
+           | Some m1, None => map2_l f m1
+           | None, Some m2 => map2_r f m2
+           end.
+      Lemma map2_l_non_empty f m : t'_P (map2_l (elt:=elt) (elt':=elt') (elt'':=elt'') f m).
+      Proof using Type.
+        clear.
+        intros _; cbv beta iota.
+        destruct (map2_l f m) as [m'|] eqn:H; [ | exact I ].
+        revert m m' H.
+        induction m as [d m pf IH] using (t_ind (elt:=_));
+          intro m'; induction m' as [d' m' pf'] using (t_case (elt:=_)).
+        all: repeat first [ match goal with
+                            | [ |- Some _ = Some _ -> _ ] => intro; inversion_option; subst
+                            | [ |- None = Some _ -> _ ] => intro; inversion_option; subst
+                            end
+                          | progress inversion_Node
+                          | progress (break_match; autounfold with trie_db; autorewrite with trie_db) ].
+        all: repeat t_non_empty_step.
+      Qed.
+      Lemma map2_r_non_empty f m : t'_P (map2_r (elt:=elt) (elt':=elt') (elt'':=elt'') f m).
+      Proof using Type.
+        clear.
+        intros _; cbv beta iota.
+        destruct (map2_r f m) as [m'|] eqn:H; [ | exact I ].
+        revert m m' H.
+        induction m as [d m pf IH] using (t_ind (elt:=_));
+          intro m'; induction m' as [d' m' pf'] using (t_case (elt:=_)).
+        all: repeat first [ match goal with
+                            | [ |- Some _ = Some _ -> _ ] => intro; inversion_option; subst
+                            | [ |- None = Some _ -> _ ] => intro; inversion_option; subst
+                            end
+                          | progress inversion_Node
+                          | progress (break_match; autounfold with trie_db; autorewrite with trie_db) ].
+        all: repeat t_non_empty_step.
+      Qed.
+      Lemma map2_non_empty f m1 m2 : t'_P (map2 (elt:=elt) (elt':=elt') (elt'':=elt'') f m1 m2).
+      Proof using Type.
+        clear.
+        intros _; cbv beta iota.
+        destruct (map2 f m1 m2) as [m'|] eqn:H; [ | exact I ].
+        revert m1 m2 m' H.
+        induction m1 as [d1 m1 pf1 IH1] using (t_ind (elt:=_));
+          intro m2; induction m2 as [d2 m2 pf2] using (t_case (elt:=_));
+          intro m'; induction m' as [d' m' pf'] using (t_case (elt:=_)).
+        all: repeat first [ match goal with
+                            | [ |- Some _ = Some _ -> _ ] => intro; inversion_option; subst
+                            | [ |- None = Some _ -> _ ] => intro; inversion_option; subst
+                            end
+                          | progress inversion_Node
+                          | progress (break_match; autounfold with trie_db; autorewrite with trie_db) ].
+        all: repeat t_non_empty_step.
+        all: lazymatch goal with
+             | [ H : map2_l ?f ?m = Some _ |- _ ]
+               => generalize (@map2_l_non_empty f m I); rewrite H; clear H
+             | [ H : map2_r ?f ?m = Some _ |- _ ]
+               => generalize (@map2_r_non_empty f m I); rewrite H; clear H
+             end.
+        all: trivial.
+      Qed.
+      Lemma map2'_non_empty f m1 m2 : t'_P (map2' f m1 m2).
+      Proof using Type.
+        clear.
+        intros _; cbv beta iota.
+        destruct m1 as [m1|], m2 as [m2|]; cbn [map2'];
+          try first [ apply map2_l_non_empty | apply map2_r_non_empty | apply map2_non_empty ]; exact I.
+      Qed.
+      Definition map2 (f : option elt -> option elt' -> option elt'') (m1 : t elt) (m2 : t elt') : t elt''
+        := mk (map2' f (proj1_sig m1) (proj1_sig m2)) (map2'_non_empty _ _ _ I).
+
+      Definition fold' A (f : key -> elt -> A -> A) (m : t' elt) (a : A) : A
+        := match m with
+           | None => a
+           | Some m => fold f m a
+           end.
+      Definition fold A (f : key -> elt -> A -> A) (m : t elt) (a : A) : A
+        := fold' f (proj1_sig m) a.
+      Definition elements_with_key_prefix_and (m : t' elt) (k_prefix : key) prefix : list (key*elt)
+        := List.rev_append (fold' (fun k v rest => (k_prefix ++ k, v) :: rest) m prefix) nil.
+      Definition elements' (m : t' elt) : list (key*elt) := elements_with_key_prefix_and m nil nil.
+      Definition elements (m : t elt) : list (key*elt) := elements' (proj1_sig m).
+      Definition cardinal (m : t elt) : nat := List.length (elements m).
+    End Types.
+
+    Definition equal elt (cmp : elt -> elt -> bool) (m1 m2 : t elt) : bool
+      := let cmp' x y
+           := match x, y with
+              | Some x, Some y => Some (cmp x y)
+              | Some _, None
+              | None, Some _
+                => Some false
+              | None, None => None
+              end in
+         fold (fun _ => andb) (map2 cmp' m1 m2) true.
+    Definition MapsTo elt (k : key) (v : elt) (m : t elt) : Prop
+      := find k m = Some v.
+    Definition eq_key elt (p p':key*elt) := E.eq (fst p) (fst p').
+    Definition eq_key_elt elt (p p':key*elt) :=
+      E.eq (fst p) (fst p') /\ (snd p) = (snd p').
+
+    Definition In elt (k : key) (m : t elt) := exists e, MapsTo k e m.
+    Definition Empty elt (m : t elt) := forall a e, ~ MapsTo a e m.
+    Definition Equal elt (m m' : t elt) := forall y, find y m = find y m'.
+    Definition Equiv elt (eq_elt:elt->elt->Prop) m m' :=
+      (forall k, In k m <-> In k m') /\
+        (forall k e e', MapsTo k e m -> MapsTo k e' m' -> eq_elt e e').
+    Definition Equivb elt (cmp: elt->elt->bool) := Equiv (Cmp cmp).
 
     Create HintDb list_map_alt discriminated.
     Create HintDb list_map_alt1 discriminated.
@@ -751,6 +727,7 @@ Module ListWSfun_gen (Y : DecidableTypeOrig) (M : WSfun Y) (Import T : Trie Y M)
                      | [ H : ?T, H' : ?T |- _ ] => clear H
                      | [ H : ?x = Some _, H' : context[?x] |- _ ] => rewrite H in H'
                      | [ H : ?x = None, H' : context[?x] |- _ ] => rewrite H in H'
+                     | [ H : proj1_sig ?x = _ |- _ ] => is_var x; destruct x
                      | [ H : Some _ = ?x |- _ ] => symmetry in H
                      | [ H : None = ?x |- _ ] => symmetry in H
                      end
@@ -762,129 +739,49 @@ Module ListWSfun_gen (Y : DecidableTypeOrig) (M : WSfun Y) (Import T : Trie Y M)
                    | progress specialize_under_binders_by progress autorewrite with list_map_alt
                    | progress cbn in * ].
 
-  Definition Empty_alt elt (m : t elt) : Prop := m = None.
-    (*Definition In_alt elt (k : key) (m : t elt) : Prop := liftKT_ (@M.In elt) (@M2.In elt).
-    Definition Equal_alt elt (m m' : t elt) : Prop := M.Equal (fst m) (fst m') /\ M2.Equal (snd m) (snd m').*)
-    Definition Equiv_alt elt (cmp : elt -> elt -> Prop) : t elt -> t elt -> Prop
-      := option_eq
-           (fun m m'
-            => t_case_nd
-                 (fun d m _
-                  => t_case_nd
-                       (fun d' m' _
-                        => option_eq cmp d d'
-                           /\ option_eq (fun m m' => M.Equiv (fun m m' => Equiv cmp (Some m) (Some m')) (`m) (`m')) m m')
-                       m')
-                 m).
-    (*Definition Equivb_alt elt (cmp : elt -> elt -> bool) (m m' : t elt) : Prop := M.Equivb cmp (fst m) (fst m') /\ M2.Equivb cmp (snd m) (snd m').
-     *)
+    Lemma find'_None elt k : @find' elt k None = None.
+    Proof. case k; t. Qed.
+    Hint Rewrite find'_None : list_map_alt.
+    Lemma find_None elt k pf : @find elt k (mk None pf) = None.
+    Proof. case k; t. Qed.
+    Hint Rewrite find_None : list_map_alt.
 
-  (*  Lemma In_alt_iff elt k (s : t elt) : In k s <-> In_alt k s.
-    Proof. t_alt_iff. Qed.
-    Lemma Equal_alt_iff elt (s s' : t elt) : Equal s s' <-> Equal_alt s s'.
-    Proof. t_alt_iff. Qed.*)
+    Definition Empty_alt elt (m : t elt) : Prop := proj1_sig m = None.
+
     Lemma Empty_alt_iff elt (s : t elt) : Empty s <-> Empty_alt s.
     Proof.
-      cbv [Empty Empty_alt MapsTo M.Empty not key M.key E.t].
-      split; repeat intro; destruct_head' t; try reflexivity; inversion_option; subst; exfalso;
+      cbv [Empty Empty_alt MapsTo M.Empty not key M.key E.t find proj1_sig].
+      split; repeat intro; destruct_head' t; destruct_head' option; try reflexivity; inversion_option;
+        exfalso;
         try solve [ destruct_one_head list; inversion_option ].
       let t := match goal with H : T.t _ |- _ => H end in
       induction t as [d m pf] using (t_ind (elt:=elt)).
-      let H := match goal with H : forall a e, find a _ = Some e -> False |- _ => H end in
+      let H := match goal with H : forall a e, find' a _ = Some e -> False |- _ => H end in
       pose proof (H nil); pose proof (fun x y => H (x :: y)); clear H.
-      cbn [find Option.bind] in *.
-      all: repeat first [ match goal with
-                          | [ H : M.Empty ?m -> False |- _ ]
-                            => pose proof (@M.elements_1 _ m);
-                               pose proof (@M.elements_2 _ m);
-                               cbv [M.Empty] in H;
-                               destruct (M.elements m)
-                          | [ H : context[InA _ _ nil] |- _ ] => setoid_rewrite InA_nil in H
-                          end
-                        | progress in_hyp_under_binders_do (fun H => rewrite InA_nil in H)
-                        | progress cbv [impl M.eq_key_elt] in *
-                        | progress specialize_by assumption
-                        | progress specialize_under_binders_by eapply InA_cons_hd
-                        | progress specialize_under_binders_by apply conj
-                        | assumption
-                        | rewrite M_find_iff in *
-                        | progress specialize_under_binders_by rewrite M_find_iff
-                        | progress t
-                        | progress specialize_under_binders_by eassumption
-                        | match goal with
-                          | [ H : ?x = Some _ |- _ ] => progress specialize_under_binders_by rewrite H
-                          end ].
+      cbn [find' Option.bind] in *.
+      repeat (autounfold with trie_db in *; autorewrite with trie_db in * ).
+      specialize_under_binders_by rewrite t_case_beta.
+      repeat t_non_empty_step.
+      let rec tac _ :=
+        first [ t_non_empty_step
+              | match goal with
+                | [ H : _ = Some _ |- _ ]
+                  => progress specialize_under_binders_by rewrite H;
+                     solve [ repeat tac () ]
+                | [ H : _ |- _ ] => apply H; clear H; solve [ repeat tac () ]
+                end ] in
+      tac ().
     Qed.
-    (*Lemma Equiv_alt_iff elt eq_elt (s s' : t elt) : Equiv eq_elt s s' <-> Equiv_alt eq_elt s s'.
+
+    Local Instance eq_key_equiv elt : Equivalence (@eq_key elt) | 10.
     Proof.
-      cbv [Equiv Equiv_alt MapsTo In M.Equiv M2.Equiv M.In M2.In key M.key M2.key not].
-      setoid_rewrite M_find_iff; setoid_rewrite M2_find_iff.
-      split; [ pose I as FWD | pose I as BAK ].
-      all: repeat first [ progress intros
-                        | progress destruct_head'_sig
-                        | progress destruct_head'_ex
-                        | progress destruct_head'_and
-                        | progress split_iff
-                        | progress specialize_dep_under_binders_by apply pair
-                        | progress specialize_dep_under_binders_by eexists
-                        | progress cbn [fst snd proj1_sig] in *
-                        | apply conj
-                        | match goal with
-                          | [ |- context[@M.find ?a ?b ?c] ] => destruct (@M.find a b c) eqn:?
-                          | [ |- context[@M2.find ?a ?b ?c] ] => destruct (@M2.find a b c) eqn:?
-                          end
-                        | solve [ eauto ]
-                        | congruence
-                        | progress specialize_under_binders_by eassumption ].
-      all: lazymatch goal with
-           | [ H : forall t e, M2.find t ?m = Some e -> ex _, H' : M2.Empty ?m -> False |- _ ]
-             => specialize (fun t e H' => H t e ltac:(apply M2.find_1, M2.elements_2, H'));
-                let H'' := fresh in
-                let H''' := fresh in
-                pose proof H' as H'';
-                cbv [M2.Empty not] in H'';
-                specialize (fun (H''' : forall a e, ~ _) => H'' (fun a e pf => ltac:(eapply (H''' a e), M2.elements_1, pf)));
-                setoid_rewrite InA_alt in H'';
-                cbv [not M2.eq_key_elt] in H'';
-                destruct (M2.elements m);
-                cbn [List.In] in H'';
-                [ specialize (H'' ltac:(firstorder tauto));
-                  exfalso; assumption
-                | specialize_under_binders_by eapply InA_cons_hd ]
-           end.
-      all: repeat first [ progress cbv [M2.eq_key_elt] in *
-                        | progress cbn [fst snd proj1_sig] in *
-                        | progress destruct_head'_sig
-                        | progress destruct_head'_ex
-                        | progress destruct_head'_and
-                        | progress specialize_dep_under_binders_by apply conj
-                        | progress specialize_dep_under_binders_by reflexivity
-                        | congruence ].
-    Qed.*)
+      split; cbv; intros; break_innermost_match; break_innermost_match_hyps; try ((idtac + symmetry + etransitivity + exfalso); (eassumption + reflexivity)).
+    Qed.
+    Local Instance eq_key_elt_equiv elt : Equivalence (@eq_key_elt elt) | 10.
+    Proof.
+      split; cbv; intros; break_innermost_match; break_innermost_match_hyps; destruct_head'_and; split; try ((idtac + symmetry + etransitivity + exfalso); (eassumption + reflexivity)).
+    Qed.
 
-    Local Ltac Proper_equiv_t :=
-      cbv;
-      setoid_rewrite M_find_iff;
-      repeat split; intros; subst; split_and; eauto.
-
-    Local Instance Proper_M_Equiv_eq_impl elt
-      : Proper ((eq ==> eq ==> impl) ==> eq ==> eq ==> impl) (@M.Equiv elt) | 10.
-    Proof. Proper_equiv_t. Qed.
-    Local Instance Proper_M_Equiv_eq_flip_impl elt
-      : Proper ((eq ==> eq ==> flip impl) ==> eq ==> eq ==> flip impl) (@M.Equiv elt) | 10.
-    Proof. Proper_equiv_t. Qed.
-    Local Instance Proper_M_Equiv_eq_iff elt
-      : Proper ((eq ==> eq ==> iff) ==> eq ==> eq ==> iff) (@M.Equiv elt) | 10.
-    Proof. Proper_equiv_t. Qed.
-    Local Instance Proper_M_Equiv_eq_impl_pointwise elt
-      : Proper (pointwise_relation _ (pointwise_relation _ impl) ==> eq ==> eq ==> impl) (@M.Equiv elt) | 10.
-    Proof. Proper_equiv_t. Qed.
-    Local Instance Proper_M_Equiv_eq_flip_impl_pointwise elt
-      : Proper (pointwise_relation _ (pointwise_relation _ (flip impl)) ==> eq ==> eq ==> flip impl) (@M.Equiv elt) | 10.
-    Proof. Proper_equiv_t. Qed.
-    Local Instance Proper_M_Equiv_eq_iff_pointwise elt
-      : Proper (pointwise_relation _ (pointwise_relation _ iff) ==> eq ==> eq ==> iff) (@M.Equiv elt) | 10.
-    Proof. Proper_equiv_t. Qed.
 
     Global
       Hint Unfold
@@ -907,7 +804,7 @@ Module ListWSfun_gen (Y : DecidableTypeOrig) (M : WSfun Y) (Import T : Trie Y M)
       In
       Empty
       Empty_alt
-      Equiv_alt
+      (*Equiv_alt*)
       (*Equivb_alt*)
       eq_key
       eq_key_elt
@@ -1067,6 +964,7 @@ Module ListWSfun_gen (Y : DecidableTypeOrig) (M : WSfun Y) (Import T : Trie Y M)
       first [ progress intros
             | t_destr_step
             | reflexivity
+            | progress destruct_head' t
             | progress destruct_head' key
             | t_specialize_safe_step ].
     Local Ltac spec_t_nosubst_step :=
@@ -1111,10 +1009,6 @@ Module ListWSfun_gen (Y : DecidableTypeOrig) (M : WSfun Y) (Import T : Trie Y M)
 
     Local Ltac spec_t := repeat spec_t_step.
 
-    Lemma find_None elt k : @find elt k None = None.
-    Proof. case k; t. Qed.
-    Hint Rewrite find_None : list_map_alt.
-
     Section Spec.
 
       Variable elt:Type.
@@ -1125,16 +1019,18 @@ Module ListWSfun_gen (Y : DecidableTypeOrig) (M : WSfun Y) (Import T : Trie Y M)
       Lemma MapsTo_1 : E.eq x y -> MapsTo x e m -> MapsTo y e m.
       Proof using Type.
         clear.
-        revert x y m.
-        induction x as [|x' xs IH], y as [|y' ys], m as [m'|]; clear x y m;
+        cbv [MapsTo find].
+        destruct m as [m' pf]; cbn [proj1_sig]; clear m pf.
+        revert x y m'.
+        induction x as [|x' xs IH], y as [|y' ys], m' as [m|]; clear x y m';
           try specialize (IH ys);
-          try (induction m' as [d m] using (t_case (elt:=elt)); clear m').
+          try (induction m as [d m'] using (t_case (elt:=elt)); clear m).
         all: t.
         all: pose_MapsTo_as_find M.MapsTo_1.
         all: repeat match goal with
-                    | [ H : context[find _ (@M.find ?a ?b ?c)] |- _ ]
+                    | [ H : context[find' _ (@M.find ?a ?b ?c)] |- _ ]
                       => destruct (@M.find a b c) eqn:?
-                    | [ |- context[find _ (@M.find ?a ?b ?c)] ]
+                    | [ |- context[find' _ (@M.find ?a ?b ?c)] ]
                       => destruct (@M.find a b c) eqn:?
                     end.
         all: specialize_under_binders_by eassumption.
@@ -1150,6 +1046,8 @@ Module ListWSfun_gen (Y : DecidableTypeOrig) (M : WSfun Y) (Import T : Trie Y M)
       Proof using Type. clear; pose proof M.is_empty_1; spec_t. Qed.
       Lemma is_empty_2 : is_empty m = true -> Empty m.
       Proof using Type. clear; pose proof M.is_empty_2; spec_t. Qed.
+      Lemma find'_iff elt0 k v m0 : @MapsTo elt0 k v m0 <-> find' k (proj1_sig m0) = Some v.
+      Proof using Type. clear; spec_t. Qed.
       Lemma find_iff elt0 k v m0 : @MapsTo elt0 k v m0 <-> find k m0 = Some v.
       Proof using Type. clear; spec_t. Qed.
       Lemma find_1 : MapsTo x e m -> find x m = Some e.
@@ -1157,16 +1055,16 @@ Module ListWSfun_gen (Y : DecidableTypeOrig) (M : WSfun Y) (Import T : Trie Y M)
       Lemma find_2 : find x m = Some e -> MapsTo x e m.
       Proof using Type. apply find_iff. Qed.
       Hint Rewrite fold_left_flat_map fold_left_map : list_map_alt.
-      Lemma elements_alt_1 (m0 : t elt) k_prefix i : elements_with_key_prefix_and m0 k_prefix (List.rev i) = fold (fun k v rest => rest ++ [(k_prefix ++ k, v)]) m0 i.
+      Lemma elements_alt_1 (m0 : t' elt) k_prefix i : elements_with_key_prefix_and m0 k_prefix (List.rev i) = fold' (fun k v rest => rest ++ [(k_prefix ++ k, v)]) m0 i.
       Proof using Type.
         clear.
         pose proof (_ : forall A, Proper (eq ==> eq ==> eq) (@cons A)).
-        cbv [elements elements_with_key_prefix_and fold].
+        cbv [elements elements_with_key_prefix_and fold'].
         rewrite <- rev_alt; destruct m0 as [m'|]; [ | rewrite rev_involutive; reflexivity ].
         revert i k_prefix.
-        induction m' as [d [m pf'] pf IH] using (t_ind (elt:=elt)); clear m'; intros.
+        induction m' as [d m pf IH] using (t_ind (elt:=elt)); clear m'; intros.
         repeat (autounfold with trie_db; autorewrite with trie_db).
-        cbn [proj1_sig] in *; clear pf'.
+        destruct m; try (now destruct d; cbn [List.rev]; rewrite rev_involutive); [].
         rewrite !M.fold_1.
         setoid_rewrite (@app_cons_app_app _ k_prefix).
         etransitivity;
@@ -1187,19 +1085,19 @@ Module ListWSfun_gen (Y : DecidableTypeOrig) (M : WSfun Y) (Import T : Trie Y M)
         induction ls as [|? ? IH]; cbn [fold_left]; intros;
           [ | rewrite <- IH ]; now rewrite rev_involutive.
       Qed.
-      Lemma elements_with_key_prefix_and_cps_id (m0 : t elt) k_prefix prefix : elements_with_key_prefix_and m0 k_prefix prefix = (List.rev prefix) ++ elements_with_key_prefix_and m0 k_prefix nil.
+      Lemma elements_with_key_prefix_and_cps_id (m0 : t' elt) k_prefix prefix : elements_with_key_prefix_and m0 k_prefix prefix = (List.rev prefix) ++ elements_with_key_prefix_and m0 k_prefix nil.
       Proof using Type.
         clear.
         pose proof (_ : forall A, Proper (eq ==> eq ==> eq) (@cons A)).
         set (n := nil); change n with (List.rev n); subst n.
         rewrite <- (List.rev_involutive prefix), !elements_alt_1, List.rev_involutive.
-        cbv [fold].
+        cbv [fold'].
         destruct m0 as [m'|]; [ | now rewrite ?app_nil_r ].
         generalize (List.rev prefix); clear prefix; intro prefix.
         revert prefix k_prefix.
-        induction m' as [d [m pf'] pf IH] using (t_ind (elt:=elt)); clear m'; intros.
+        induction m' as [d m pf IH] using (t_ind (elt:=elt)); clear m'; intros.
         repeat (autounfold with trie_db; autorewrite with trie_db).
-        cbn [proj1_sig] in *; clear pf'.
+        destruct m; try (now destruct d; rewrite ?app_nil_r, ?app_nil_l); [].
         rewrite !M.fold_1.
         setoid_rewrite (@app_cons_app_app _ k_prefix).
         etransitivity;
@@ -1228,7 +1126,7 @@ Module ListWSfun_gen (Y : DecidableTypeOrig) (M : WSfun Y) (Import T : Trie Y M)
           [ reflexivity | ].
         now rewrite <- IH, ?app_assoc.
       Qed.
-      Lemma elements_with_key_prefix_alt (m0 : t elt) k_prefix prefix
+      Lemma elements_with_key_prefix_alt (m0 : t' elt) k_prefix prefix
         : elements_with_key_prefix_and m0 k_prefix (List.rev prefix)
           = prefix
               ++ match m0 with
@@ -1243,7 +1141,7 @@ Module ListWSfun_gen (Y : DecidableTypeOrig) (M : WSfun Y) (Import T : Trie Y M)
                               ++ (List.flat_map
                                     (fun km => elements_with_key_prefix_and (Some (snd km)) (k_prefix ++ [fst km]) nil)
                                     match m with
-                                    | Some (exist m _) => M.elements m
+                                    | Some m => M.elements m
                                     | None => []
                                     end))
                         m
@@ -1255,11 +1153,11 @@ Module ListWSfun_gen (Y : DecidableTypeOrig) (M : WSfun Y) (Import T : Trie Y M)
         apply f_equal.
         change (@nil ?A) with (List.rev (@nil A)) at 1.
         rewrite elements_alt_1.
-        cbv [fold].
+        cbv [fold'].
         destruct m0 as [m'|]; [ | now rewrite ?app_nil_r ].
         induction m' as [d m pf] using (t_case (elt:=elt)); clear m'.
         repeat (autounfold with trie_db; autorewrite with trie_db).
-        destruct m as [[m' _]|]; [ | break_innermost_match; cbn; now rewrite ?app_nil_r ].
+        destruct m as [m'|]; [ | break_innermost_match; cbn; now rewrite ?app_nil_r ].
         cbn [List.app].
         clear pf.
         set (d' := match d with None => nil | Some _ => _ end).
@@ -1274,15 +1172,15 @@ Module ListWSfun_gen (Y : DecidableTypeOrig) (M : WSfun Y) (Import T : Trie Y M)
         apply f_equal2; [ | reflexivity ].
         rewrite <- (List.rev_involutive d'), <- elements_with_key_prefix_and_cps_id, elements_alt_1, rev_involutive; reflexivity.
       Qed.
-      Lemma map_elements_with_key_prefix_and k_prefix (m0 : t elt)
+      Lemma map_elements_with_key_prefix_and k_prefix (m0 : t' elt)
         : List.map
             (fun '(ks, v) => (k_prefix ++ ks, v))
-            (elements m0)
+            (elements' m0)
           = elements_with_key_prefix_and m0 k_prefix nil.
       Proof using Type.
         clear.
         pose proof (_ : forall A, Proper (eq ==> eq ==> eq) (@cons A)).
-        cbv [elements].
+        cbv [elements'].
         set (i := nil) at 2 3.
         etransitivity; [ | set_evars; rewrite <- (app_nil_r k_prefix); subst_evars; reflexivity ].
         set (k_prefix' := nil).
@@ -1295,9 +1193,9 @@ Module ListWSfun_gen (Y : DecidableTypeOrig) (M : WSfun Y) (Import T : Trie Y M)
         clearbody i k_prefix'.
         clear.
         revert k_prefix k_prefix'.
-        induction m' as [d [m pf'] pf IH] using (t_ind (elt:=elt)); clear m'; intros.
+        induction m' as [d m pf IH] using (t_ind (elt:=elt)); clear m'; intros.
         repeat (autounfold with trie_db; autorewrite with trie_db).
-        cbn [proj1_sig] in *; clear pf'.
+        destruct m as [m'|]; [ | break_innermost_match; cbn; now rewrite ?app_nil_r ].
         rewrite map_app.
         apply f_equal2;
           [ now break_innermost_match; cbn; rewrite ?app_nil_r
@@ -1311,8 +1209,8 @@ Module ListWSfun_gen (Y : DecidableTypeOrig) (M : WSfun Y) (Import T : Trie Y M)
         specialize_under_binders_by (rewrite InA_alt; eexists; split; try eassumption; repeat split; try apply Y.eq_refl).
         eapply IH; eassumption.
       Qed.
-      Lemma elements_alt (m0 : t elt)
-        : elements m0
+      Lemma elements'_alt (m0 : t' elt)
+        : elements' m0
           = match m0 with
             | None => []
             | Some m
@@ -1325,18 +1223,18 @@ Module ListWSfun_gen (Y : DecidableTypeOrig) (M : WSfun Y) (Import T : Trie Y M)
                          ++ (List.flat_map
                                (fun '(k, m) => List.map
                                                  (fun '(ks, v) => (k :: ks, v))
-                                                 (elements (Some m)))
+                                                 (elements' (Some m)))
                                match m with
-                               | Some (exist m _) => M.elements m
+                               | Some m => M.elements m
                                | None => []
                                end))
                    m
             end.
       Proof using Type.
         clear.
-        unfold elements at 1.
+        unfold elements' at 1.
         change (@nil ?A) with (List.rev (@nil A)) at 2.
-        rewrite elements_with_key_prefix_alt; cbn -[elements].
+        rewrite elements_with_key_prefix_alt; cbn -[elements'].
         destruct m0 as [m'|]; [ | reflexivity ].
         induction m' as [d m pf] using (t_case (elt:=elt)); clear m'.
         repeat (autounfold with trie_db; autorewrite with trie_db).
@@ -1351,16 +1249,16 @@ Module ListWSfun_gen (Y : DecidableTypeOrig) (M : WSfun Y) (Import T : Trie Y M)
       Proof using Type.
         clear.
         intros A i f.
-        cbv [fold].
-        destruct m as [m'|]; clear m; [ | reflexivity ].
+        cbv [fold fold' elements].
+        destruct m as [[m'|] pf']; clear m; [ | reflexivity ].
+        cbn [proj1_sig] in *; clear pf'.
         revert f i.
         induction m' as [d m pf IH] using (t_ind (elt:=elt)); clear m'; intros.
-        specialize_under_binders_by (apply M.find_1, M.elements_2; rewrite InA_alt; eexists; repeat split; try reflexivity).
-        rewrite elements_alt.
+        rewrite elements'_alt.
         repeat (autounfold with trie_db; autorewrite with trie_db).
+        destruct m as [m'|]; [ | now break_innermost_match ].
+        specialize_under_binders_by (apply M.find_1, M.elements_2; rewrite InA_alt; eexists; repeat split; try reflexivity).
         clear pf.
-        destruct m as [m' pf']; clear m.
-        cbn [proj1_sig] in *; clear pf'.
         rewrite M.fold_1.
         rewrite fold_left_app, fold_left_flat_map.
         etransitivity; [ apply fold_left_ext_in | f_equal; try reflexivity; break_innermost_match; cbn; reflexivity ]; cbn.
@@ -1370,37 +1268,21 @@ Module ListWSfun_gen (Y : DecidableTypeOrig) (M : WSfun Y) (Import T : Trie Y M)
         rewrite fold_left_map; f_equiv; repeat intro; subst; break_innermost_match; reflexivity.
       Qed.
 
-      Lemma M_add_full elt0 m0 v x' y' : @M.find elt0 y' (M.add x' v m0) = if Y.eq_dec x' y' then Some v else M.find y' m0.
+      Lemma add'_full m0 v x' y' : @find' elt y' (Some (add' x' v m0)) = if E.eq_dec x' y' then Some v else find' y' m0.
       Proof using Type.
         clear.
-        pose_MapsTo_as_find M.add_1.
-        pose_MapsTo_as_find M.add_2.
-        pose_MapsTo_as_find M.add_3.
-        repeat match goal with
-               | [ |- context[M.find ?x ?m] ]
-                 => destruct (M.find x m) eqn:?
-               end.
-        all: break_innermost_match.
-        all: specialize_under_binders_by eassumption.
-        all: intuition congruence.
-      Qed.
-      Hint Rewrite M_add_full : list_map_alt.
-      Lemma add_full m0 v x' y' : @find elt y' (add x' v m0) = if E.eq_dec x' y' then Some v else find y' m0.
-      Proof using Type.
-        clear.
-        cbv [add].
         revert x' y' m0.
         induction x' as [|x xs IH], y' as [|y ys], m0 as [m|];
           first [ specialize (IH ys) | try clear IH ];
           try (induction m as [d m'] using (t_case (elt:=elt)); clear m).
         all: repeat first [ progress invlist eqlistA
-                          | progress cbn [find add' Option.bind]
+                          | progress cbn [find' add' Option.bind]
                           | progress cbv [not] in *
                           | progress autounfold with trie_db
                           | reflexivity
                           | progress specialize_under_binders_by apply eqlistA_cons
                           | match goal with
-                            | [ IH : forall m, find ?k (Some (add' ?xs ?v m)) = _ |- context[find ?k (Some (add' ?xs ?v ?m'))] ]
+                            | [ IH : forall m, find' ?k (Some (add' ?xs ?v m)) = _ |- context[find' ?k (Some (add' ?xs ?v ?m'))] ]
                               => rewrite IH
                             end
                           | progress break_innermost_match_step
@@ -1409,24 +1291,13 @@ Module ListWSfun_gen (Y : DecidableTypeOrig) (M : WSfun Y) (Import T : Trie Y M)
         all: t.
       Qed.
       Lemma add_1 : E.eq x y -> MapsTo y e (add x e m).
-      Proof using Type. clear; intros; rewrite !find_iff, !add_full in *; spec_t. Qed.
+      Proof using Type. clear; cbv [find add]; intros; rewrite !find'_iff, !add'_full in *; spec_t. Qed.
       Lemma add_2 : ~ E.eq x y -> MapsTo y e m -> MapsTo y e (add x e' m).
-      Proof using Type. clear; intros; rewrite !find_iff, !add_full in *; spec_t. Qed.
+      Proof using Type. clear; cbv [find add]; intros; rewrite !find'_iff, !add'_full in *; spec_t. Qed.
       Lemma add_3 : ~ E.eq x y -> MapsTo y e (add x e' m) -> MapsTo y e m.
-      Proof using Type. clear; intros; rewrite !find_iff, !add_full in *; spec_t. Qed.
-      Lemma M_remove_full elt0 m0 x' y' : @M.find elt0 y' (M.remove x' m0) = if Y.eq_dec x' y' then None else M.find y' m0.
-      Proof using Type.
-        clear.
-        pose proof (@M.remove_1 elt0 m0 x' y').
-        pose proof (@M.remove_2 elt0 m0 x' y').
-        pose proof (@M.remove_3 elt0 m0 x' y').
-        cbv [M.In] in *.
-        spec_t.
-        specialize_under_binders_by reflexivity; spec_t.
-      Qed.
-      Hint Rewrite M_remove_full : list_map_alt.
-      Lemma remove_full m0 x' y'
-        : @find elt y' (remove x' m0) = if E.eq_dec x' y' then None else find y' m0.
+      Proof using Type. clear; cbv [find add]; intros; rewrite !find'_iff, !add'_full in *; spec_t. Qed.
+      Lemma remove'_full m0 x' y'
+        : @find' elt y' (remove' x' m0) = if E.eq_dec x' y' then None else find' y' m0.
       Proof using Type.
         clear.
         revert x' y' m0.
@@ -1438,7 +1309,7 @@ Module ListWSfun_gen (Y : DecidableTypeOrig) (M : WSfun Y) (Import T : Trie Y M)
                           | progress inversion_option
                           | progress inversion_sigma
                           | progress invlist eqlistA
-                          | progress cbn [find remove Option.bind]
+                          | progress cbn [find' remove' Option.bind]
                           | progress cbv [not] in *
                           | progress autounfold with trie_db
                           | progress split_iff
@@ -1448,14 +1319,12 @@ Module ListWSfun_gen (Y : DecidableTypeOrig) (M : WSfun Y) (Import T : Trie Y M)
                           | progress specialize_under_binders_by apply eqlistA_nil
                           | progress specialize_under_binders_by apply eqlistA_cons
                           | match goal with
-                            | [ H : forall m, find ?ys (remove ?xs m) = _, H' : remove ?xs _ = Some ?v |- context[Some ?v] ]
+                            | [ H : forall m, find' ?ys (remove' ?xs m) = _, H' : remove' ?xs _ = Some ?v |- context[Some ?v] ]
                               => rewrite <- H', H
-                            | [ H : forall m, find ?ys (remove ?xs m) = find ?ys m, H' : remove ?xs ?m' = None |- context[find ?ys ?m'] ]
+                            | [ H : forall m, find' ?ys (remove' ?xs m) = find' ?ys m, H' : remove' ?xs ?m' = None |- context[find' ?ys ?m'] ]
                               => rewrite <- H, H'
                             | [ H : context[@M.is_empty_1 ?a ?b] |- _ ]
                               => generalize dependent (@M.is_empty_1 a b)
-                            | [ H : context[@_TrieShape.map_is_empty_1 ?a ?b] |- _ ]
-                              => generalize dependent (@_TrieShape.map_is_empty_1 a b)
                             end
                           | progress break_innermost_match_step
                           | progress autorewrite with trie_db list_map_alt in *
@@ -1470,22 +1339,18 @@ Module ListWSfun_gen (Y : DecidableTypeOrig) (M : WSfun Y) (Import T : Trie Y M)
                                  apply M.is_empty_2 in H;
                                  cbv [M.Empty not] in H;
                                  try now exfalso
-                            | [ |- None = find _ (@M.find ?a ?b ?c) ]
+                            | [ |- None = find' _ (@M.find ?a ?b ?c) ]
                               => destruct (@M.find a b c) eqn:?
                             end ].
         all: specialize_all_ways.
         all: t.
       Qed.
       Lemma remove_1 : E.eq x y -> ~ In y (remove x m).
-      Proof using Type. clear; cbv [In]; setoid_rewrite find_iff; setoid_rewrite remove_full; spec_t. Qed.
+      Proof using Type. clear; cbv [In]; setoid_rewrite find_iff; setoid_rewrite remove'_full; spec_t. Qed.
       Lemma remove_2 : ~ E.eq x y -> MapsTo y e m -> MapsTo y e (remove x m).
-      Proof using Type. clear; cbv [In]; setoid_rewrite find_iff; setoid_rewrite remove_full; spec_t. Qed.
+      Proof using Type. clear; cbv [In]; setoid_rewrite find_iff; setoid_rewrite remove'_full; spec_t. Qed.
       Lemma remove_3 : MapsTo y e (remove x m) -> MapsTo y e m.
-      Proof using Type. clear; cbv [In]; setoid_rewrite find_iff; setoid_rewrite remove_full; spec_t. Qed.
-
-      Lemma M_elements_iff elt0 x0 e0 m0 :
-        InA (@M.eq_key_elt elt0) (x0,e0) (M.elements m0) <-> M.MapsTo x0 e0 m0.
-      Proof using Type. split; first [ apply M.elements_1 | apply M.elements_2 ]. Qed.
+      Proof using Type. clear; cbv [In]; setoid_rewrite find_iff; setoid_rewrite remove'_full; spec_t. Qed.
 
       Lemma elements_iff :
         MapsTo x e m <-> InA (@eq_key_elt _) (x,e) (elements m).
@@ -1493,17 +1358,19 @@ Module ListWSfun_gen (Y : DecidableTypeOrig) (M : WSfun Y) (Import T : Trie Y M)
         clear; cbv [MapsTo].
         rewrite InA_alt.
         cbv [eq_key_elt]; cbn [fst snd].
+        destruct m as [m' pf]; clear m.
+        cbv [find elements proj1_sig]; clear pf; rename m' into m.
         revert m; induction x as [|?? IH];
           (intros [m'|];
            [ induction m' as [d m pf] using (t_case (elt:=elt)); clear m'
-           | now rewrite elements_alt; destruct x; cbn; split; intros; inversion_option; firstorder ]).
-        all: rewrite elements_alt.
+           | now rewrite elements'_alt; destruct x; cbn; split; intros; inversion_option; firstorder ]).
+        all: rewrite elements'_alt.
         all: repeat (autounfold with trie_db; autorewrite with trie_db).
-        all: destruct m as [[m' pf']|]; cbn [proj1_sig] in *.
+        all: destruct m as [m'|].
         all: setoid_rewrite in_app_iff.
         all: setoid_rewrite in_flat_map.
-        all: cbn [find Option.bind].
-        all: repeat (autounfold with trie_db; autorewrite with trie_db).
+        all: cbn [find' Option.bind].
+        all: repeat (cbn [Option.bind]; autounfold with trie_db; autorewrite with trie_db).
         1-2: now split; intros; subst; t;
         eexists (_, _); cbn; repeat esplit; try reflexivity; eauto.
         all: try (rewrite IH; clear IH).
@@ -1530,9 +1397,9 @@ Module ListWSfun_gen (Y : DecidableTypeOrig) (M : WSfun Y) (Import T : Trie Y M)
                             | [ H : M.find _ _ = Some _ |- _ ] => apply M.find_2, M.elements_1 in H
                             | [ |- False \/ _ ] => right
                             | [ |- ((nil, _) = (cons _ _, _) \/ False) \/ _ ] => right
-                            | [ H : List.In _ (elements (M.find ?k ?m)) |- _ ]
+                            | [ H : List.In _ (elements' (M.find ?k ?m)) |- _ ]
                               => destruct (M.find k m) eqn:?
-                            | [ H : context[elements None] |- _ ]
+                            | [ H : context[elements' None] |- _ ]
                               => cbn in H
                             end
                           | eexists (_, _)
@@ -1547,12 +1414,13 @@ Module ListWSfun_gen (Y : DecidableTypeOrig) (M : WSfun Y) (Import T : Trie Y M)
       Lemma elements_3w : NoDupA (@eq_key _) (elements m).
       Proof using Type.
         clear.
-        destruct m as [m'|]; clear m; [ | now constructor ].
+        cbv [elements proj1_sig]; destruct m as [[m'|] _]; clear m;
+          [ | now constructor ].
         induction m' as [d m pf IH] using (t_ind (elt:=elt)); clear m'.
-        rewrite elements_alt.
+        rewrite elements'_alt.
         repeat (autounfold with trie_db; autorewrite with trie_db).
         apply NoDupA_app; try exact _; break_innermost_match; repeat constructor;
-          intros *; try (rewrite !InA_alt; cbv [eq_key]); destruct m as [m' pf']; clear m; cbn [fst snd List.In proj1_sig] in *; clear pf' pf.
+          intros *; try (rewrite !InA_alt; cbv [eq_key]); cbn [fst snd List.In proj1_sig] in *; clear pf.
         all: repeat first [ intro
                           | progress cbn [fst snd proj1_sig] in *
                           | progress destruct_head'_ex
@@ -1563,7 +1431,7 @@ Module ListWSfun_gen (Y : DecidableTypeOrig) (M : WSfun Y) (Import T : Trie Y M)
                           | rewrite in_flat_map in *
                           | rewrite in_map_iff in *
                           | break_innermost_match_hyps_step
-                          | progress destruct_head'_prod
+                          | progress destruct_head' prod
                           | progress setoid_subst_rel E.eq
                           | rewrite ECompat.eq_alt in *
                           | progress invlist eqlistA ].
@@ -1578,7 +1446,7 @@ Module ListWSfun_gen (Y : DecidableTypeOrig) (M : WSfun Y) (Import T : Trie Y M)
         { cbv [eq_key M.eq_key]; intros; rewrite !InA_alt in *.
           repeat match goal with
                  | [ H : context[M.elements _] |- _ ] => clear H
-                 | [ H : context[@elements ?A] |- _ ] => generalize dependent (@elements A); intros
+                 | [ H : context[@elements' ?A] |- _ ] => generalize dependent (@elements' A); intros
                  | [ H : ~M.Empty _ |- _ ] => clear H
                  | [ H : option _ |- _ ] => clear H
                  end.
@@ -1598,32 +1466,22 @@ Module ListWSfun_gen (Y : DecidableTypeOrig) (M : WSfun Y) (Import T : Trie Y M)
       Proof using Type. split; first [ apply M.equal_1 | apply M.equal_2 ]. Qed.
     End Spec.
 
-    Lemma M_mapi_full : forall (elt elt':Type)(m: M.t elt)(x:M.key)(f:M.key->elt->elt'), exists y, Y.eq y x /\ M.find x (M.mapi f m) = option_map (f y) (M.find x m).
-    Proof.
-      pose proof M.mapi_1 as H.
-      setoid_rewrite M_find_iff in H.
-      pose proof M.mapi_2 as H'.
-      cbv [M.In] in *.
-      setoid_rewrite M_find_iff in H'.
-      specialize_under_binders_by eapply ex_intro.
-      spec_t.
-      specialize_under_binders_by eassumption; spec_t.
-    Qed.
-    Hint Rewrite M_mapi_full : list_map_alt.
     Lemma mapi_full : forall (elt elt':Type)(m: t elt)(x:key)(f:key->elt->elt'), exists y, E.eq y x /\ find x (mapi f m) = option_map (f y) (find x m).
     Proof.
-      cbv [mapi].
-      intros elt elt' [m|]; [ | intros [|]; eexists; split; reflexivity ].
-      induction m as [d [m pf'] pf IH] using (t_ind (elt:=elt)).
+      cbv [mapi find].
+      intros elt elt' [[m|] pf]; [ | intros [|]; eexists; split; reflexivity ].
+      cbn [proj1_sig]; clear pf.
+      induction m as [d m pf IH] using (t_ind (elt:=elt)).
       intros [|x xs] f.
-      all: cbn [find]; cbn [option_map Option.bind].
+      all: cbn [find']; cbn [option_map Option.bind].
       all: repeat (autounfold with trie_db; autorewrite with trie_db).
       all: try (eexists; split; reflexivity).
       all: [ > ].
-      cbn [option_map proj1_sig] in *.
-      clear pf pf'.
+      destruct m as [m|]; [ | now cbn; eauto ].
+      cbn [option_map proj1_sig Option.bind] in *.
+      clear pf.
       edestruct M_mapi_full as [? [HY H]]; rewrite H.
-      destruct (M.find x m) eqn:H'; rewrite ?find_None; cbn [option_map] in *.
+      destruct (M.find x m) eqn:H'; rewrite ?find'_None; cbn [option_map] in *.
       1: specialize_under_binders_by eassumption.
       1: do 2 (let t := open_constr:(_) in evar (v : t); specialize (IH v); subst v).
       1: destruct IH as [? [? IH]].
@@ -1663,62 +1521,38 @@ Module ListWSfun_gen (Y : DecidableTypeOrig) (M : WSfun Y) (Import T : Trie Y M)
       edestruct mapi_full as [?[? ->]].
       destruct find; cbn; intros; repeat t_destr_step; eauto.
     Qed.
-    Lemma M_map2_full
-      : forall (elt elt' elt'':Type)(m: M.t elt)(m': M.t elt')
-	       (x:M.key)(f:option elt->option elt'->option elt''),
-        M.find x (M.map2 f m m') = match M.find x m, M.find x m' with
-                                   | None, None => None
-                                   | x, y => f x y
-                                   end.
-    Proof.
-      intros *.
-      pose proof (@M.map2_1 elt elt' elt'' m m' x f) as H.
-      pose proof (@M.map2_2 elt elt' elt'' m m' x f) as H'.
-      cbv [M.In] in *.
-      setoid_rewrite M_find_iff in H.
-      setoid_rewrite M_find_iff in H'.
-      specialize_under_binders_by eapply ex_intro.
-      destruct (M.find x (M.map2 f m m')); break_innermost_match; try reflexivity;
-        specialize_by eauto; specialize_under_binders_by reflexivity; eauto.
-      firstorder congruence.
-    Qed.
-    Lemma map2_full
-      : forall (elt elt' elt'':Type)(m: t elt)(m': t elt')
+    Lemma map2'_full
+      : forall (elt elt' elt'':Type)(m: t' elt)(m': t' elt')
 	       (x:key)(f:option elt->option elt'->option elt''),
-        find x (map2 f m m') = match find x m, find x m' with
-                               | None, None => None
-                               | x, y => f x y
-                               end.
+        find' x (map2' f m m') = match find' x m, find' x m' with
+                                 | None, None => None
+                                 | x, y => f x y
+                                 end.
     Proof.
       intros elt elt' elt'' m m' x f.
       revert m m'.
       induction x as [|x xs IH].
-      { cbv [map2 find Option.bind]; intros.
+      { cbv [map2' find' Option.bind]; intros.
         repeat first [ t_destr_conj_step
                      | reflexivity
                      | break_innermost_match_step
                      | break_innermost_match_hyps_step
                      | progress break_match_hyps
                      | progress autounfold with trie_db in *
+                     | progress inversion_Node
                      | match goal with
-                       | [ H : Node _ _ _ = Node _ _ _ |- _ ]
-                         => let H' := fresh in
-                            pose proof (f_equal (t_case_nd (fun d m pf => (d, m))) H) as H';
-                            clear H;
-                            cbv [t_case_nd] in *;
-                            autorewrite with trie_db in H'
                        | [ |- context[t_case _ ?v] ]
                          => is_var v; induction v using (t_case (elt:=_));
                             autorewrite with trie_db in *
                        end
                      | progress autorewrite with trie_db in * ]. }
       intros [m|] [m'|]; try reflexivity;
-        try induction m as [d [[m pfm]|] pf] using (t_case (elt:=elt));
-        try induction m' as [d' [[m' pfm']|] pf'] using (t_case (elt:=elt'));
+        try induction m as [d [m|] pf] using (t_case (elt:=elt));
+        try induction m' as [d' [m'|] pf'] using (t_case (elt:=elt'));
         first [ specialize (IH (M.find x m)) | specialize (IH None) ];
         first [ specialize (IH (M.find x m')) | specialize (IH None) ].
-      all: rewrite ?find_None in *.
-      all: cbn [find]; cbv [map2 Option.bind] in *.
+      all: rewrite ?find'_None in *.
+      all: cbn [find']; cbv [map2' Option.bind] in *.
       all: repeat first [ reflexivity
                         | progress repeat (autounfold with trie_db in *; autorewrite with trie_db in * )
                         | progress break_match
@@ -1729,18 +1563,10 @@ Module ListWSfun_gen (Y : DecidableTypeOrig) (M : WSfun Y) (Import T : Trie Y M)
                           end ].
       all: repeat first [ t_destr_conj_step
                         | reflexivity
+                        | progress inversion_Node
                         | match goal with
-                          | [ H : Node _ _ _ = Node _ _ _ |- _ ]
-                            => let H' := fresh in
-                               pose proof (f_equal (t_case_nd (fun d m pf => (d, m))) H) as H';
-                               clear H;
-                               cbv [t_case_nd] in *;
-                               autorewrite with trie_db in H'
-                          | [ H : dec_empty_cps _ _ _ = Some _ |- _ ]
-                            => pose proof (dec_empty_Some H); clear H
-                          | [ H : dec_empty_cps _ _ _ = None |- _ ]
-                            => apply dec_empty_None in H
-                          | [ H : M.is_empty _ = true |- _ ] => apply M.is_empty_2 in H
+                          | [ H : M.is_empty _ = true |- _ ]
+                            => apply M.is_empty_2 in H
                           | [ H : M.Empty (M.map2 _ _ _) |- _ ]
                             => cbv [M.Empty not] in H;
                                setoid_rewrite M_find_iff in H;
@@ -1762,7 +1588,7 @@ Module ListWSfun_gen (Y : DecidableTypeOrig) (M : WSfun Y) (Import T : Trie Y M)
                         | rewrite M_map2_full
                         | rewrite map_xgmap2_l by reflexivity
                         | rewrite map_xgmap2_r by reflexivity
-                        | rewrite find_None in *
+                        | rewrite find'_None in *
                         | break_innermost_match_step
                         | break_innermost_match_hyps_step
                         | progress break_match_hyps
@@ -1775,8 +1601,10 @@ Module ListWSfun_gen (Y : DecidableTypeOrig) (M : WSfun Y) (Import T : Trie Y M)
         find x (map2 f m m') = f (find x m) (find x m').
     Proof.
       cbv [In]; intros *.
-      setoid_rewrite find_iff.
-      rewrite !map2_full.
+      setoid_rewrite find'_iff.
+      cbv [find map2 proj1_sig]; intros *.
+      destruct m as [m _], m' as [m' _].
+      rewrite !map2'_full.
       break_innermost_match; try reflexivity.
       firstorder congruence.
     Qed.
@@ -1786,8 +1614,10 @@ Module ListWSfun_gen (Y : DecidableTypeOrig) (M : WSfun Y) (Import T : Trie Y M)
         In x (map2 f m m') -> In x m \/ In x m'.
     Proof.
       cbv [In]; intros *.
-      setoid_rewrite find_iff.
-      rewrite !map2_full.
+      setoid_rewrite find'_iff.
+      cbv [find map2 proj1_sig]; intros *.
+      destruct m as [m _], m' as [m' _].
+      rewrite !map2'_full.
       break_innermost_match; firstorder; inversion_option; eauto.
     Qed.
 
@@ -1826,7 +1656,8 @@ Module ListWSfun_gen (Y : DecidableTypeOrig) (M : WSfun Y) (Import T : Trie Y M)
                     eexists; repeat esplit; try eassumption; reflexivity
                   | clear H ]
              end.
-        all: specialize_under_binders_by (apply elements_1, find_2; rewrite map2_full).
+        all: specialize_under_binders_by (apply elements_1, find_2; setoid_rewrite map2'_full).
+        all: destruct_head' t; cbv [proj1_sig find] in *.
         all: repeat match goal with
                     | [ H : _ = Some _ |- _ ]
                       => progress specialize_under_binders_by rewrite H
@@ -1842,13 +1673,14 @@ Module ListWSfun_gen (Y : DecidableTypeOrig) (M : WSfun Y) (Import T : Trie Y M)
         all: lazymatch goal with
              | [ H : InA _ _ (elements (map2 _ _ _)) |- _ ]
                => apply elements_2, find_1 in H;
-                  rewrite map2_full in H
+                  setoid_rewrite map2'_full in H
              end.
+        all: cbv [proj1_sig] in *.
         all: break_innermost_match_hyps; specialize_under_binders_by eapply ex_intro.
         all: specialize_under_binders_by reflexivity.
         all: repeat t_destr_conj_step.
         all: specialize_under_binders_by eassumption.
-        eassumption.
+        all: eassumption.
       Qed.
       Lemma equal_1 : Equivb cmp m m' -> equal cmp m m' = true.
       Proof using Type. apply equal_iff. Qed.
@@ -1913,10 +1745,13 @@ Module ListSfun_gen (Y : OrderedTypeOrig) (M : Sfun Y) (Import T : Trie Y M).
       Proof using Type.
         pose proof Y'.lt_compat.
         pose proof P'.lt_compat.
-        destruct m as [m|]; [ | constructor ].
-        induction m as [d [m pfm] pf IH] using (t_ind (elt:=elt)).
-        rewrite elements_alt.
+        destruct m as [[m|] pfm]; [ | constructor ].
+        cbv [elements proj1_sig].
+        clear pfm.
+        induction m as [d m pf IH] using (t_ind (elt:=elt)).
+        rewrite elements'_alt.
         repeat (autounfold with trie_db; autorewrite with trie_db).
+        destruct m as [m|]; [ | now break_innermost_match; cbn; repeat constructor ].
         eapply @SortA_app with (eqA:=@eq_key_elt _); try exact _.
         all: try solve [ break_innermost_match; repeat constructor ].
         all: try solve [
