src/Util/FSets/FMapTrie/Shape.v
@@ -1,0 +1,371 @@
+Require Import Coq.Bool.Bool.
+Require Import Coq.Lists.List.
+Require Import Coq.Structures.Orders.
+Require Import Coq.Structures.OrdersEx.
+Require Import Coq.FSets.FMapInterface.
+Require Import Coq.Classes.RelationPairs.
+Require Import Crypto.Util.Option.
+Require Import Crypto.Util.Prod.
+Require Import Crypto.Util.ListUtil.
+Require Import Crypto.Util.ListUtil.SetoidList.
+Require Import Crypto.Util.ListUtil.SetoidListFlatMap.
+Require Import Crypto.Util.ListUtil.StdlibCompat.
+Require Import Crypto.Util.Tactics.SpecializeBy.
+Require Import Crypto.Util.Tactics.DestructHead.
+Require Import Crypto.Util.Tactics.SpecializeUnderBindersBy.
+
+Local Set Implicit Arguments.
+Local Set Primitive Projections.
+Local Unset Strict Implicit.
+(* TODO: move to global settings *)
+Local Set Keyed Unification.
+Import ListNotations.
+Local Open Scope option_scope.
+Local Open Scope bool_scope.
+Local Open Scope lazy_bool_scope.
+Local Open Scope type_scope.
+Local Open Scope list_scope.
+
+Module Type TypFunctor.
+  Parameter t : Type -> Type.
+End TypFunctor.
+
+Module Import EverythingGen.
+  Polymorphic Definition id_fix {T} (x : T) := x.
+  Polymorphic Definition id_fix_2 {T} (x : T) := x.
+  Polymorphic Definition id_case {T} (x : T) := x.
+  Section __.
+    Context (t : Type -> Type)
+            (map_key : Type)
+            (map_t : Type -> Type)
+            (map_empty : forall elt, map_t elt)
+            (map_is_empty : forall elt, map_t elt -> bool)
+            (map_fold : forall elt A : Type, (map_key -> elt -> A -> A) -> map_t elt -> A -> A)
+            (map_mapi : forall elt elt' : Type, (map_key -> elt -> elt') -> map_t elt -> map_t elt')
+            (map_map2 : forall elt elt' elt'' : Type, (option elt -> option elt' -> option elt'') -> map_t elt -> map_t elt' -> map_t elt'')
+            (map_find : forall elt : Type, map_key -> map_t elt -> option elt).
+
+    Local Notation t' elt := (option (t elt)).
+    Local Notation node_NonEmpty x y := match x, y with None, None => False | _, _ => True end.
+    Local Notation node_NonEmpty' x y := match y, x with None, None => False | _, _ => True end.
+    Local Notation map_t_t elt := (map_t (t elt)).
+
+    Section step.
+      Context (Node : forall elt (d : option elt) (m : option (map_t_t elt)), node_NonEmpty d m -> t elt)
+              (t_case_nd : forall (elt : Type) (P : Type),
+                  (forall (v : option elt) (m : option (map_t_t elt)), node_NonEmpty v m -> P)
+                  -> t elt -> P)
+              (map_xmap2_l : forall elt elt' elt'', (option elt -> option elt' -> option elt'') -> map_t elt -> map_t elt'')
+              (map_xmap2_r : forall elt elt' elt'', (option elt -> option elt' -> option elt'') -> map_t elt' -> map_t elt'').
+
+      Local Arguments Node {_} _ _ _.
+
+      Definition empty' : forall elt, t' elt
+        := fun _ => None.
+
+      Definition mapi_step elt elt'
+                 (mapi : (list map_key -> elt -> elt') -> t elt -> t elt')
+                 (f : list map_key -> elt -> elt')
+        : t elt -> t elt'
+        := let d_of d := option_map (f nil) d in
+           let m_of m
+             := option_map
+                  (@map_mapi _ _ (fun k => mapi (fun ks => f (k :: ks))))
+                  m in
+           t_case_nd
+             (fun d m pf
+              => Node
+                   (d_of d) (m_of m)
+                   (match d, m return node_NonEmpty d m -> node_NonEmpty (d_of d) (m_of m) with
+                    | None, None => fun pf => pf
+                    | _, _ => fun 'I => I
+                    end pf)).
+
+      Local Notation dec_empty m := (if map_is_empty m then None else Some m).
+
+      Definition map2_step
+                 elt elt' elt'' (f : option elt -> option elt' -> option elt'')
+                 (map2_l : t elt -> t' elt'')
+                 (map2_r : t elt' -> t' elt'')
+                 (map2 : t elt -> t elt' -> t' elt'')
+                 (m1 : t elt) (m2 : t elt')
+        : t' elt''
+        := let F := (fun m1 m2
+                     => match m1, m2 with
+                        | Some m1, Some m2 => map2 m1 m2
+                        | Some m1, None => map2_l m1
+                        | None, Some m2 => map2_r m2
+                        | None, None => None
+                        end) in
+           let f' x y := match x, y with
+                         | None, None => None
+                         | x, y => f x y
+                         end in
+           t_case_nd
+             (fun d1 m1 pf1
+              => t_case_nd
+                   (fun d2 m2 pf2
+                    => let m := match m1, m2 with
+                                | Some m1, Some m2
+                                  => dec_empty (@map_map2 _ _ _ F m1 m2)
+                                | Some m1, None
+                                  => dec_empty (map_xmap2_l F m1)
+                                | None, Some m2
+                                  => dec_empty (map_xmap2_r F m2)
+                                | None, None => None
+                                end in
+                       match f' d1 d2, m with
+                       | None, None => None
+                       | d, m => Some (Node d m I)
+                       end)
+                   m2)
+             m1.
+      Definition map2_l_step
+                 elt elt' elt'' (f : option elt -> option elt' -> option elt'')
+                 (map2_l : t elt -> t' elt'')
+                 (m1 : t elt)
+        : t' elt''
+        := let f' x y := match x, y with
+                         | None, None => None
+                         | x, y => f x y
+                         end in
+           t_case_nd
+             (fun d1 m1 pf1
+              => let m := match m1 with
+                          | Some m1
+                            => dec_empty
+                                 (@map_xmap2_l
+                                    (t elt) (t elt') (t elt'')
+                                    (fun m1 _ => match m1 with
+                                                 | None => None
+                                                 | Some m1 => map2_l m1
+                                                 end)
+                                    m1)
+                          | None => None
+                          end in
+                 match f' d1 None, m with
+                 | None, None => None
+                 | d, m => Some (Node d m I)
+                 end)
+             m1.
+      Definition map2_r_step
+                 elt elt' elt'' (f : option elt -> option elt' -> option elt'')
+                 (map2_r : t elt' -> t' elt'')
+                 (m2 : t elt')
+        : t' elt''
+        := let f' x y := match x, y with
+                         | None, None => None
+                         | x, y => f x y
+                         end in
+           t_case_nd
+             (fun d2 m2 pf2
+              => let m := match m2 with
+                          | Some m2
+                            => dec_empty
+                                 (@map_xmap2_r
+                                    (t elt) (t elt') (t elt'')
+                                    (fun _ m2 => match m2 with
+                                                 | None => None
+                                                 | Some m2 => map2_r m2
+                                                 end)
+                                    m2)
+                          | None => None
+                          end in
+                 match f' None d2, m with
+                 | None, None => None
+                 | d, m => Some (Node d m I)
+                 end)
+             m2.
+      Definition fold_step elt A
+                 (fold : (list map_key -> elt -> A -> A) -> t elt -> A -> A)
+                 (f : list map_key -> elt -> A -> A)
+                 (m : t elt)
+                 (a : A)
+        : A
+        := t_case_nd
+             (fun d m pf
+              => let a := match d with
+                          | None => a
+                          | Some d => f [] d a
+                          end in
+                 match m with
+                 | Some m
+                   => @map_fold
+                        _ _
+                        (fun k => fold (fun ks => f (k :: ks)))
+                        m
+                        a
+                 | None => a
+                 end)
+             m.
+      Definition recursively_non_empty_step elt
+                 (recursively_non_empty : t elt -> bool)
+                 (m : t elt)
+        : bool
+        := t_case_nd
+             (fun d m pf
+              => match m with
+                 | Some m
+                   => @map_fold
+                        _ _
+                        (fun _ m P => andb P (recursively_non_empty m))
+                        m
+                        (negb (map_is_empty m))
+                 | None => true
+                 end)
+             m.
+    End step.
+
+    Class EverythingGen
+      := { Node : forall elt (d : option elt) (m : option (map_t_t elt)), node_NonEmpty d m -> t elt
+         ; t_case : forall elt (P : t elt -> Type),
+             (forall d m pf, P (@Node elt d m pf))
+             -> forall m, P m
+         ; t_case_beta : forall elt P rec d m pf, @t_case elt P rec (@Node elt d m pf) = rec d m pf
+         ; t_case_nd
+           := fun elt P => @t_case elt (fun _ => P)
+         ; t_ind : forall elt (P : t elt -> Prop),
+             (forall d m pf, (forall k v, match m with Some m => @map_find _ k m = Some v -> P v | None => True end) -> P (@Node elt d m pf))
+             -> forall m, P m
+         ; empty : forall elt, t' elt
+           := fun _ => None
+         ; mapi : forall elt elt', id_fix_2 ((list map_key -> elt -> elt') -> t elt -> t elt')
+         ; mapi_beta : forall elt elt' f m, @mapi elt elt' f m = mapi_step Node t_case_nd (@mapi elt elt') f m
+
+         ; map_xmap2_l : forall elt elt' elt'', (option elt -> option elt' -> option elt'') -> map_t elt -> map_t elt''
+         ; map_xmap2_r : forall elt elt' elt'', (option elt -> option elt' -> option elt'') -> map_t elt' -> map_t elt''
+         ; map_xmap2_lr : forall A B (f g : option A -> option A -> option B) m,
+             (forall i j, f i j = g j i) -> map_xmap2_l f m = map_xmap2_r g m
+         ; map_xgmap2_l : forall A B C (f : option A -> option B -> option C) i m,
+             f None None = None -> @map_find _ i (map_xmap2_l f m) = f (@map_find _ i m) None
+         ; map_xgmap2_r : forall A B C (f : option A -> option B -> option C) i m,
+             f None None = None -> @map_find _ i (map_xmap2_r f m) = f None (@map_find _ i m)
+
+         ; map2_l : forall elt elt' elt'', (option elt -> option elt' -> option elt'') -> id_fix (t elt -> t' elt'')
+         ; map2_r : forall elt elt' elt'', (option elt -> option elt' -> option elt'') -> id_fix (t elt' -> t' elt'')
+         ; map2 : forall elt elt' elt'', (option elt -> option elt' -> option elt'') -> id_fix (t elt -> t elt' -> t' elt'')
+         ; map2_l_beta : forall elt elt' elt'' f m,
+             @map2_l elt elt' elt'' f m = map2_l_step Node t_case_nd map_xmap2_l f (map2_l f) m
+         ; map2_r_beta : forall elt elt' elt'' f m,
+             @map2_r elt elt' elt'' f m = map2_r_step Node t_case_nd map_xmap2_r f (map2_r f) m
+         ; map2_beta : forall elt elt' elt'' f m1 m2,
+             @map2 elt elt' elt'' f m1 m2 = map2_step Node t_case_nd map_xmap2_l map_xmap2_r f (map2_l f) (map2_r f) (map2 f) m1 m2
+         ; fold : forall elt (A : Type), id_fix_2 ((list map_key -> elt -> A -> A) -> t elt -> A -> A)
+         ; fold_beta : forall elt A f m a,
+             @fold elt A f m a = fold_step t_case_nd (@fold elt A) f m a
+         ; recursively_non_empty : forall elt, id_fix (t elt -> bool)
+         ; recursively_non_empty_beta : forall elt m,
+             @recursively_non_empty elt m = recursively_non_empty_step t_case_nd (@recursively_non_empty elt) m
+      }.
+    Definition Node' {E : EverythingGen} elt (d : option elt) (m : option (map_t_t elt)) : node_NonEmpty' d m -> t elt
+      := match d, m return node_NonEmpty' d m -> _ with
+         | None, None => fun pf => match pf with end
+         | d, (Some _ | None) as m => @Node E elt d m
+         end.
+    Definition oNode_dec_empty {E : EverythingGen} elt (d : option elt) (m : map_t (t elt)) : option (t elt)
+      := match d, (if map_is_empty m then None else Some m) with
+         | None, None => None
+         | d, (None | Some _) as m
+           => Some (Node (d:=d) (m:=m) I)
+         end.
+  End __.
+End EverythingGen.
+Global Arguments Node {t _ _ _ _ _ _ _ _ _} d m _.
+Global Arguments Node' {t _ _ _ _ _ _ _ _ _} d m _.
+
+Create HintDb trie_db discriminated.
+
+Hint Rewrite
+     t_case_beta
+     mapi_beta
+     map2_beta
+     map2_l_beta
+     map2_r_beta
+     fold_beta
+     recursively_non_empty_beta
+  : trie_db.
+
+Hint Unfold
+     id_fix
+     id_fix_2
+     id_case
+     Node'
+     oNode_dec_empty
+     empty'
+     mapi_step
+     map2_step
+     map2_l_step
+     map2_r_step
+     fold_step
+     recursively_non_empty_step
+     t_case_nd
+     empty
+  : trie_db.
+
+Module Type TrieShape (label : DecidableType) (map : FMapInterface.WSfun label) (Import T : TypFunctor).
+  Notation Everything := (@EverythingGen t map.key map.t map.is_empty map.fold map.mapi map.map2 map.find).
+End TrieShape.
+
+Module Type Trie (label : DecidableType) (map : FMapInterface.WSfun label).
+  Include TypFunctor.
+  Include TrieShape label map.
+  Parameter Inline everything : Everything.
+  Existing Instance everything.
+End Trie.
+
+Module TrieTactics.
+  Ltac t_destr_conj_step :=
+    first [ progress subst
+          | progress destruct_head'_False
+          | progress destruct_head'_and
+          | progress destruct_head'_ex
+          | progress destruct_head'_True
+          | progress destruct_head'_unit
+          | progress destruct_head' sig
+          | progress inversion_option
+          | progress inversion_sigma
+          | progress inversion_list
+          | progress inversion_pair
+          | progress cbn [fst snd proj1_sig proj2_sig] in *
+          | match goal with
+            | [ H : eqlistA _ nil _ |- _ ] => inversion H; clear H
+            | [ H : eqlistA _ _ nil |- _ ] => inversion H; clear H
+            | [ H : eqlistA _ (_ :: _) _ |- _ ] => inversion H; clear H
+            | [ H : eqlistA _ _ (_ :: _) |- _ ] => inversion H; clear H
+            | [ H : InA _ _ (_ :: _) |- _ ] => inversion H; clear H
+            | [ H : InA _ _ nil |- _ ] => inversion H; clear H
+            | [ H : List.In _ (List.map _ _) |- _ ] => rewrite in_map_iff in H
+            | [ H : List.In _ (List.flat_map _ _) |- _ ] => rewrite in_flat_map in H
+            | [ H : ?x = ?x |- _ ] => clear H
+            | [ H : ?T, H' : ?T |- _ ] => clear H
+            | [ H : ?x = Some _, H' : context[?x] |- _ ] => rewrite H in H'
+            | [ H : ?x = None, H' : context[?x] |- _ ] => rewrite H in H'
+            | [ H : Some _ = ?x |- _ ] => symmetry in H
+            | [ H : None = ?x |- _ ] => symmetry in H
+            end
+          | discriminate ].
+  Ltac t_destr_step :=
+    first [ t_destr_conj_step
+          | progress destruct_head'_or
+          | progress destruct_head' option
+          | break_innermost_match_hyps_step
+          | break_innermost_match_step ].
+  Ltac t_specialize_safe_step :=
+    first [ progress specialize_by_assumption
+          | progress cbv [not] in *
+          | progress specialize_by reflexivity
+          | progress specialize_under_binders_by apply conj
+          | progress specialize_under_binders_by eapply ex_intro
+          | progress specialize_under_binders_by apply eqlistA_cons ].
+
+  Ltac inversion_Node_step :=
+    match goal with
+    | [ H : Node _ _ _ = Node _ _ _ |- _ ]
+      => let H' := fresh in
+         pose proof (f_equal (t_case_nd (fun d m pf => (d, m))) H) as H';
+         clear H;
+         cbv [t_case_nd] in *;
+         autorewrite with trie_db in H'
+    end.
+  Ltac inversion_Node := repeat inversion_Node_step.
+End TrieTactics.
